Almost no skips for permutation proofs in label-free, part of ppermut lib completed

NormalizationProperties.v
@@ -3,6 +3,7 @@ Require Import Labeled.
 Require Import Metatheory.
 Require Import List.
 Require Import Relations.
+Require Import Arith.
 
 Open Scope labeled_is5_scope.
 
@@ -21,16 +22,11 @@ Inductive neutral: te_L -> Prop :=
 Lemma neutral_or_value:
 forall M,
   neutral M \/ value_L M.
-induction M; intros.
-left; constructor.
-right; constructor.
-left; constructor.
-right; constructor.
-left; constructor.
-left; constructor.
-left; constructor.
-destruct IHM; [left | right]; constructor; auto.
-left; constructor.
+induction M; intros; 
+try (destruct IHM; [left | right]; constructor; auto);
+try (left; constructor);
+right;
+constructor.
 Qed.
 
 (*
@@ -78,7 +74,7 @@ Qed.
 
 (* We want to have the property that term that has a type is strongly normalizing *)
 Inductive strong_norm: te_L -> var -> Prop :=
-| val_SN: forall M w, value_L M -> strong_norm M w
+| val_SN: forall M, value_L M -> forall w, strong_norm M w
 | step_SN: forall M w, 
              (forall N, (M, fwo w) |-> (N, fwo w) -> strong_norm N w) -> 
              strong_norm M w.
@@ -176,7 +172,7 @@ match A with
 end.
 
 (* CR 2 base *)
-Theorem head_expansion:
+Theorem property_2:
 forall w A M M'
   (HRed: Reducible M A w)
   (H_lc: lc_w M)
@@ -202,8 +198,7 @@ forall A M w
   (H_lc: lc_w M),
   (Reducible M A w -> strong_norm M w)
   /\
-  ( neutral M -> 
-   (forall M', (M, fwo w) |-> (M', fwo w) -> Reducible M' A w) ->
+  ( neutral M -> (forall M', (M, fwo w) |-> (M', fwo w) -> Reducible M' A w) ->
    Reducible M A w).
 induction A; intros; split; simpl in *.
 (* base type *)
@@ -246,12 +241,172 @@ intro; contradiction.
 skip. (* not finished *)
 Qed.
 
+Lemma property_1:
+forall A M w
+  (H_lc: lc_w M),
+  Reducible M A w -> strong_norm M w.
+intros; eapply reducibility_props; eauto.
+Qed.
+
+Lemma property_3:
+forall A M w
+  (H_lc: lc_w M),
+  neutral M -> 
+  (forall M', (M, fwo w) |-> (M', fwo w) -> 
+    Reducible M' A w) ->
+   Reducible M A w.
+intros; eapply reducibility_props; eauto.
+Qed.
+
+Fixpoint red_ctx (D: list te_L) (Gamma: list (ty_L * wo)) :=
+match (D, Gamma) with
+| (nil, nil) => True
+| (M :: D', (A, fwo w):: Gamma') => Reducible M A w /\ red_ctx D' Gamma'
+| (_, _) => False
+end.
+
+Lemma reducible_abstraction:
+forall A w N B
+  (lc_N: lc_w N)
+  (HT: forall M, 
+    Reducible M A w ->
+    Reducible ([M//0] N) B w),
+  Reducible (lam_L A N) (A ---> B) w.
+simpl; intros.
+apply property_3.
+repeat constructor; auto.
+constructor.
+intros.
+inversion H; subst.
+apply HT; auto.
+inversion HRed.
+Qed.
+
+(* Extra substitution properties - FIXME: move *)
+Lemma subst_list_var:
+forall D Omega Gamma n m A w
+  (HT: nth_error Gamma n = Some (A, fwo w))
+  (HT': subst_typing Omega D Gamma),
+  nth_error D n = Some (subst_list D m (hyp_L (n + m))) /\
+  Omega; nil |- subst_list D m (hyp_L (n + m)) ::: A @ w.
+induction D; intros; inversion Gamma; subst; skip.
+Qed.
+
+Lemma subst_list_lam:
+forall D n A M,
+  subst_list D n (lam_L A M) = lam_L A (subst_list D (S n) M).
+Admitted.
+
+Lemma subst_list_appl:
+forall D n M N,
+  subst_list D n (appl_L M N) = appl_L (subst_list D n M) (subst_list D n N).
+Admitted.
+
+Lemma subst_list_box:
+forall D n M,
+  subst_list D n (box_L M) = box_L (subst_list D n M).
+Admitted.
+
+Lemma subst_list_unbox:
+forall D n M,
+  subst_list D n (unbox_L M) = unbox_L (subst_list D n M).
+Admitted.
+
+Lemma subst_list_get:
+forall D n M w ,
+  subst_list D n (get_L w M) = get_L w (subst_list D n M).
+Admitted.
+
+Lemma subst_list_fetch:
+forall D n M w ,
+  subst_list D n (fetch_L w M) = fetch_L w (subst_list D n M).
+Admitted.
+
+Lemma subst_list_here:
+forall D n M,
+  subst_list D n (here_L M) = here_L (subst_list D n M).
+Admitted.
+
+Lemma subst_list_letd:
+forall D n M N,
+  subst_list D n (letd_L M N) = letd_L (subst_list D n M) (subst_list D (S n) M).
+Admitted.
+
+Lemma subst_hyp_gt:
+forall D n,
+  subst_list D (S n) (hyp_L n) = hyp_L n.
+Admitted.
+
+Lemma subst_hyp:
+forall Omega Gamma D n A w M,
+  Omega; Gamma |- hyp_L n ::: A @ w ->
+  nth_error D n = Some M ->
+  subst_list D 0 (hyp_L n) = M.
+Admitted.
+
+Lemma lc_w_subst_list:
+forall D M k,
+  (forall N, In N D -> lc_w N) ->
+  lc_w M ->
+  lc_w (subst_list D k M).
+Admitted.  
+(* / End *)
+
+Theorem subst_types_reducible:
+forall M Omega Gamma A w D
+  (H_lc: lc_w M)
+  (H_lc_D: forall N, In N D -> lc_w N)
+  (HT: Omega; Gamma |- M ::: A @ w)
+  (HRed: red_ctx D Gamma),
+  Reducible (subst_list D 0 M) A w.
+induction M; intros; inversion HT; subst.
+(* hyp : TODO *)
+assert (exists M, nth_error D n = Some M) by skip.
+destruct H as (M).
+assert (Reducible M A w) by skip.
+assert (subst_list D 0 (hyp_L n) = M) by (eapply subst_hyp; eauto).
+subst; auto.
+(* lam *)
+rewrite subst_list_lam.
+apply reducible_abstraction.
+inversion H_lc; subst; apply lc_w_subst_list; auto.
+intros.
+specialize IHM with 
+  (Omega:=Omega)(Gamma:=(t, fwo w)::Gamma) 
+  (A:=A') (w:=w) (D:= M0 :: D).
+simpl in IHM.
+apply IHM.
+inversion H_lc; subst; auto.
+intros; destruct H0; subst; auto.
+skip. (* details... *)
+assumption.
+split; auto.
+(* appl *)
+inversion H_lc; subst.
+assert (Reducible (subst_list D 0 M1) (A'--->A) w) by
+  (eapply IHM1; eauto).
+simpl in H.
+rewrite subst_list_appl.
+apply H.
+apply lc_w_subst_list; auto.
+eapply IHM2; eauto.
+(* box *)
+(* unbox *)
+(* get *)
+(* letd *)
+(* here *)
+(* fetch *)
+Admitted.
+
+
 Theorem types_reducible:
 forall Omega M A w,
   lc_w M ->
   Omega; nil |- M ::: A @ w ->
     Reducible M A w.
-Admitted.
+intros; apply subst_types_reducible with (D:=nil) in H0; 
+simpl in *; intros; eauto; contradiction.
+Qed.
 
 Theorem strong_normalization_theorem:
 forall Omega M A w,
