PermutationLib.v
@@ -1,0 +1,282 @@
+Require Export Shared.
+Require Import LibListSorted.
+Require Import Setoid.
+Require Import LibList.
+
+Inductive PPermut: list Context_LF -> list Context_LF -> Prop :=
+| PPermut_nil: PPermut nil nil
+| PPermut_skip: forall G G' w Gamma Gamma', 
+    permut Gamma Gamma' ->
+    PPermut G G' ->
+    PPermut ((w, Gamma)::G) ((w,Gamma')::G')
+| PPermut_swap: forall G w w' Gamma0 Gamma0' Gamma1 Gamma1',
+    permut Gamma0 Gamma1 ->
+    permut Gamma0' Gamma1' ->
+    PPermut ((w, Gamma0) :: (w', Gamma0') :: G)
+                ((w', Gamma1') :: (w, Gamma1) :: G)
+| PPermut_trans: forall G G' G'',
+    PPermut G G' -> PPermut G' G'' -> PPermut G G''.
+Hint Constructors PPermut.
+
+Notation "G ~=~ G'" := (PPermut G G') (at level 70) : ppermut_scope. 
+Notation " Ctx *=* Ctx'" := (permut Ctx Ctx') (at level 70) : ppermut_scope.
+
+Open Scope ppermut_scope.
+
+Lemma PPermut_reflexive:
+  Reflexive PPermut.
+unfold Reflexive; intros;
+induction x;
+  [ | destruct a]; 
+  eauto.
+Qed. 
+
+Lemma PPermut_symmetric:
+  Symmetric PPermut.
+unfold Symmetric; intros;
+induction H; eauto.
+  apply PPermut_trans with (G':=(w, Gamma')::G); eauto;
+  apply PPermut_skip;
+  [ apply permut_sym | 
+    apply PPermut_reflexive];
+  auto.
+  apply PPermut_swap; apply permut_sym; assumption.
+Qed.
+
+Lemma PPermut_transitive:
+  Transitive PPermut.
+exact PPermut_trans.
+Qed.  
+
+Hint Resolve PPermut_reflexive.
+
+Theorem PPermut'oid: Setoid_Theory _ PPermut.
+  split.
+  exact PPermut_reflexive.
+  exact PPermut_symmetric.
+  exact PPermut_transitive.
+Qed.
+
+Add Setoid (list Context_LF) PPermut PPermut'oid as PPermutoid.
+
+Lemma test1:
+  forall G, PPermut G G.
+auto.
+Qed.
+
+Add Morphism (@cons Context_LF) : PPermut_cons.
+intro y; destruct y; auto.
+Qed.
+Hint Resolve PPermut_cons.
+
+Lemma test2:
+  forall G G' w Gamma, PPermut G G' -> PPermut ((w, Gamma)::G) ((w, Gamma) :: G').
+auto.
+Qed.
+
+Lemma test3:
+  forall G G' w Gamma, PPermut G G' -> PPermut ((w, Gamma)::G') ((w, Gamma) :: G).
+intros;
+apply PPermutoid;
+auto.
+Qed.
+
+Lemma PPermut_app_tail:
+forall G G' G0,
+  G ~=~ G' ->
+  G ++ G0 ~=~ G' ++ G0.
+intros; induction H; simpl; rew_app; auto;
+econstructor; eauto.
+Qed.
+
+Lemma PPermut_app_head:
+forall G0 G G',
+  G ~=~ G' ->
+  G0 ++ G ~=~ G0 ++ G'.
+intros; induction G0; simpl; rew_app; auto.
+Qed.
+Hint Resolve PPermut_app_tail PPermut_app_head.
+
+Add Morphism (@append Context_LF) : PPermut_app.
+intros; induction H; simpl in *; rew_app; auto.
+transitivity ((w, Gamma0) :: (w', Gamma0') :: G ++ y0); auto.
+transitivity (G' ++ y0); auto.
+Qed.
+Hint Resolve PPermut_app.
+
+Lemma test4:
+forall G G' G'' G0 G1 Ctx,
+  G ~=~ G' ->
+  G0 ~=~ G1 ->
+  G ++ Ctx :: G'' ++ G0 ~=~ G' ++ Ctx :: G'' ++ G1.
+auto.
+Qed.
+
+Theorem PPermut_app_comm:
+forall G1 G2,
+  G1 ++ G2 ~=~ G2 ++ G1.
+induction G1; intros; simpl; rew_app;
+[ auto |
+ induction G2]; simpl in *.
+rewrite app_nil_r; auto.
+destruct a; destruct a0;
+transitivity ((v,l) :: (v0, l0) :: G2 ++ G1).
+constructor; auto; apply IHG1.
+transitivity ((v0, l0) :: (v, l) :: G2 ++ G1); auto;
+constructor; auto;
+transitivity ((v,l) :: G1 ++ G2); auto;
+constructor; [ | apply PPermutoid] ; auto.
+Qed.
+Hint Resolve PPermut_app_comm.
+
+Lemma test5:
+forall G G' G'' G0 G1,
+  G ~=~ G' ->
+  G0 ~=~ G1 ->
+  G0 ++ G ++ G'' ~=~ G' ++ G1 ++ G''.
+intros; transitivity (G ++ G0 ++ G'');
+repeat rewrite <- app_assoc; auto.
+Qed.
+
+Theorem PPermut_cons_app:
+forall G2 G1 G3 a,
+  G1 ~=~ G2 ++ G3 ->
+  a :: G1 ~=~ G2 ++ a :: G3.
+induction G2; intros; simpl in *; rew_app; auto;
+transitivity (a0 :: a :: G2 ++ G3); auto;
+transitivity (a :: a0 :: G2 ++ G3); auto;
+destruct a; destruct a0; auto.
+Qed.
+Hint Resolve PPermut_cons_app.
+
+Theorem PPermut_middle:
+forall G1 G2 a,
+  a :: G1 ++ G2 ~=~ G1 ++ a :: G2.
+auto.
+Qed.
+
+Lemma PPermut_nil_impl:
+forall L,
+  nil ~=~ L -> L = nil.
+intros; remember (@nil Context_LF) as L' in H;
+induction H; intros;
+discriminate || auto.
+Qed.
+
+Lemma PPermut_nil_contr:
+forall L a,
+  ~ (PPermut nil (a::L)).
+induction L; intros; intro;
+apply PPermut_nil_impl in H; discriminate.
+Qed.
+
+Hint Resolve PPermut_nil_impl PPermut_nil_contr.
+
+Lemma PPermut_last_simpl:
+forall L L' a, 
+  L ~=~ L' ->
+  L & a ~=~ L' & a.
+intros; apply PPermut_app_tail; auto.
+Qed.
+
+Lemma PPermut_last:
+forall L L' w t t',
+  t *=* t' ->
+  L ~=~ L' ->
+  L & (w, t) ~=~ L' & (w, t').
+induction L; destruct L'; intros; simpl;
+auto.
+Qed.
+
+Hint Resolve PPermut_last_simpl PPermut_last.
+
+Lemma PPermut_mid_last_app:
+forall G' G G0,
+  G ++ G' ~=~ G0 ->
+  forall a,
+    G & a ++ G' ~=~ G0 & a.
+intros; rew_app;
+transitivity (a:: nil ++ G0);
+[ simpl; apply PPermut_symmetric in H; apply PPermut_symmetric | ];
+auto.
+Qed.
+Hint Resolve PPermut_mid_last_app.
+
+Lemma PPermut_cons_last_same:
+forall L a,
+  a :: L ~=~ L & a.
+induction L; intros;
+[ | rew_app]; auto.
+transitivity (a :: a0 :: L); [destruct a0; destruct a | ]; auto.
+Qed.
+
+Lemma PPermut_cons_last:
+forall L L' a,
+  L ~=~ L' ->
+  a :: L ~=~ L' & a.
+intros; rewrite H; apply PPermut_cons_last_same.
+Qed.
+Hint Resolve PPermut_cons_last_same PPermut_cons_last.
+
+Lemma PPermut_last_rev_simpl:
+forall G G' a,
+  G & a ~=~ G' & a ->
+  G ~=~ G'.
+Admitted.
+
+Lemma PPermut_last_rev:
+forall G G' w Gamma Gamma',
+  Gamma *=* Gamma' ->
+  G & (w, Gamma) ~=~ G' & (w, Gamma') ->
+  G ~=~ G'.
+Admitted.
+
+Lemma PPermut_split_neq:
+forall G G' w w' Gamma Gamma',
+  G & (w, Gamma) ~=~ G' & (w', Gamma') ->
+  ~Gamma *=* Gamma' \/ w <> w' ->
+  exists GH, exists GT, G = GH & (w', Gamma') ++ GT.
+Admitted.
+
+Lemma PPermut_middle_last:
+forall G G' C,
+  G ++ G' & C ~=~ G ++ C :: G'.
+Admitted.
+Hint Resolve PPermut_middle_last.
+
+Lemma PPermut_specialized1:
+forall G G' C C',
+  G ++ C :: G' & C' ~=~ G ++ G' ++ C' :: C :: nil.
+Admitted.
+
+Lemma PPermut_specialized2:
+forall GH GT G Gamma Gamma' Gamma'',
+  GH ++ Gamma :: GT & Gamma' ~=~ G & Gamma ->
+  GH ++ GT ++ Gamma'' :: Gamma' :: nil ~=~ G & Gamma''.
+Admitted.
+
+Lemma PPermut_specialized3:
+forall G G' C C',
+  G ++ G' ++ C :: C' :: nil ~=~ G ++ C :: G' & C'.
+Admitted.
+
+Lemma PPermut_specialized4:
+forall G GH GT Gamma Gamma0 Gamma'0,
+  GH ++ Gamma :: GT & Gamma'0 ~=~ G & Gamma ->
+  G ++ Gamma0 :: Gamma :: nil ~=~ GH ++ GT ++ Gamma0 :: Gamma'0 :: Gamma :: nil.
+Admitted.
+
+Lemma PPermut_specialized5:
+forall G G' C C' C'',
+  G ++ C :: G' ++ C' :: C'' :: nil ~=~ (G ++ G' ++ C' :: C'' :: nil) & C.
+Admitted.
+
+Lemma PPermut_specialized6:
+forall GH GT C0 C'' C'0,
+  GH ++ GT ++ C'0 :: C'' :: C0 :: nil ~=~ GH ++ GT ++ C0 :: C'0 :: C'' :: nil.
+Admitted.
+
+Hint Resolve PPermut_specialized1 PPermut_specialized2 PPermut_specialized3 PPermut_specialized4.
+Hint Resolve PPermut_specialized5 PPermut_specialized6.
+Close Scope ppermut_scope.
+
