Shared.v
@@ -1,0 +1,89 @@
+Require Import Metatheory.
+
+(* Definitions *)
+
+(* 
+Types in IS5 system:
+   * base type
+   * arrow type for functions
+   * box type for universally true terms
+   * diamond type for existentially true terms
+*)
+Inductive ty :=
+| tvar: ty
+| tarrow: ty -> ty -> ty
+| tbox: ty -> ty
+| tdia: ty -> ty
+.
+Notation " A '--->' B " := (tarrow A B) 
+  (at level 30, right associativity) : is5_scope.
+Notation " '[*]' A " := (tbox A) 
+  (at level 30) : is5_scope.
+Notation " '<*>' A " := (tdia A) 
+  (at level 30) : is5_scope.
+
+(*
+Variables for worlds - bound and free
+*)
+Inductive vwo := 
+| bwo: nat -> vwo
+| fwo: var -> vwo
+.
+
+(*
+Variables for terms - bound and free
+*)
+Inductive vte :=
+| bte: nat -> vte
+| fte: var -> vte
+.
+
+(* Properties *)
+
+(* Decidability *)
+
+Theorem eq_ty_dec:
+forall a b: ty, {a = b} + {a <> b}.
+  decide equality. 
+Qed.
+
+(* 
+Decidability for var is not expressed in the library, so we need to
+assume is manually.
+*)
+Axiom eq_var_dec:
+  forall v1 v2: var, {v1 = v2} + {v1 <> v2}.
+
+Theorem eq_vwo_dec:
+forall w1 w2: vwo, {w1 = w2} + {w1 <> w2}.
+  decide equality.
+  decide equality.
+  apply eq_var_dec.
+Qed.
+
+Theorem eq_vte_dec:
+forall v1 v2: vte, {v1 = v2} + {v1 <> v2}.
+  decide equality.
+  decide equality.
+  apply eq_var_dec.
+Qed.
+
+(* Free variable extraction *)
+
+Definition var_from_vwo (w: vwo) :=
+match w with
+| fwo w0 => \{w0}
+| bwo _ => \{}
+end.
+
+Definition var_from_vte (v: vte) :=
+match v with
+| fte v0 => \{v0}
+| bte _ => \{}
+end.
+
+(* Shared definitions *)
+
+Definition Context_LF := prod var (list (prod var ty)).
+Definition Background_LF := list Context_LF.
+
