label-free/Semantics.v
@@ -1,4 +1,8 @@
 (* TODO: imports are messed up now that there's a module *) 
+Add LoadPath "./..".
+
+Require Import Utf8.
+
 Require Import Syntax.
 Require Import Substitution.
 Require Import Metatheory.
@@ -6,8 +10,11 @@ Require Import LibList.
 Require Import LibListSorted.
 Require Import Arith.
 
-Open Scope label_free_is5_scope.
+Require Import PermutationLib.
 
+Open Scope label_free_is5_scope.
+Open Scope is5_scope.
+Open Scope ppermut_scope.
 
 Fixpoint ok A (G: list (var * A)) (Used: list var) : Prop :=
 match G with 
@@ -21,11 +28,11 @@ ok (ty_LF) (flat_map snd G) nil.
 
 Global Reserved Notation " G '|=' Ctx '|-' M ':::' A " (at level 70).
  
-(* Statics *)
+(* Statics *) 
 
 Inductive types_LF: Background_LF -> Context_LF -> te_LF -> ty_LF -> Prop :=
 
-| t_hyp_LF: forall A G w Gamma v
+| t_hyp_LF: forall A G w (Gamma: list (prod var ty_LF)) v
   (Ok_Bg: ok_Bg ((w, Gamma) :: G))
   (HT: Mem (v, A) Gamma),
   G |= (w, Gamma) |- hyp_LF (fvar v) ::: A
@@ -56,7 +63,7 @@ Inductive types_LF: Background_LF -> Context_LF -> te_LF -> ty_LF -> Prop :=
 | t_unbox_fetch_LF: forall A G w Gamma w' Gamma' M
   (Ok_Bg: ok_Bg ((w, Gamma) :: G & (w', Gamma')))
   (HT: (G & (w', Gamma')) |= (w, Gamma) |- M ::: [*] A),
-  forall G', permut (G & (w, Gamma)) G' ->
+  forall G', (G & (w, Gamma)) ~=~ G' ->
     G' |= (w', Gamma') |- unbox_fetch_LF (fctx w) M ::: A
 
 | t_here_LF: forall A G w Gamma M
@@ -67,7 +74,7 @@ Inductive types_LF: Background_LF -> Context_LF -> te_LF -> ty_LF -> Prop :=
 | t_get_here_LF: forall A G w Gamma Ctx' M
   (Ok_Bg: ok_Bg ((w, Gamma) :: G & Ctx'))
   (HT: G & Ctx' |= (w, Gamma) |- M ::: A),
-  forall G', permut (G & (w, Gamma)) G' -> 
+  forall G', PPermut (G & (w, Gamma)) G' -> 
     G' |= Ctx' |- get_here_LF (fctx w) M ::: <*> A
 
 | t_letdia_LF: forall L_w L_t A B G w Gamma M N
@@ -78,13 +85,13 @@ Inductive types_LF: Background_LF -> Context_LF -> te_LF -> ty_LF -> Prop :=
       (w, Gamma) |- (N ^w^ (fctx w')) ^t^ (hyp_LF (fvar v')) ::: B),
   G |= (w, Gamma) |- letdia_get_LF (fctx w) M N ::: B 
 
-| t_letdia_get_LF: forall L_w L_t A B G w Gamma Ctx' M N
+| t_letdia_get_LF: forall L_w L_t A B G w (Gamma: list (prod var ty_LF)) Ctx' M N
   (Ok_Bg: ok_Bg ((w, Gamma) :: G & Ctx'))
   (HT1: G & Ctx' |= (w, Gamma) |- M ::: <*> A)
   (HT2: forall v', v' \notin L_t -> forall w', w' \notin L_w ->
     (w', ((v', A) :: nil)) :: G & (w, Gamma) |= 
       Ctx' |- (N ^w^ (fctx w')) ^t^ (hyp_LF (fvar v')) ::: B),
-  forall G0, permut (G & (w, Gamma)) G0 -> 
+  forall G0, PPermut (G & (w, Gamma)) G0 -> 
     G0 |= Ctx' |- letdia_get_LF (fctx w) M N ::: B
 where " G '|=' Ctx '|-' M ':::' A " := (types_LF G Ctx M A) : label_free_is5_scope.
 
@@ -147,23 +154,283 @@ exists (var_gen L);
 apply var_gen_spec.
 Qed.
 
+Lemma ContextPermutImpl:
+forall G Gamma Gamma' w M A
+  (HPerm: Gamma *=* Gamma')
+  (HT: G |= (w, Gamma) |- M ::: A),
+  G |= (w, Gamma') |- M ::: A.
+intros; generalize dependent Gamma'; induction HT;
+intros; simpl in *.
+Admitted.
+
+Lemma BackgroundSubsetImpl:
+forall G G' Ctx M A
+  (HT: G |= Ctx |- M ::: A)
+  (HSubst: exists GT, PPermut (G++GT) G'),
+  G' |= Ctx |- M ::: A.
+intros;
+generalize dependent G';
+induction HT; intros.
+(* hyp *)
+constructor; auto. skip.
+(* appl *)
+econstructor; eauto. skip.
+(* lam *)
+econstructor; eauto. skip.
+(* box *)
+destruct HSubst as [GT];
+apply t_box_LF with (L:=L); intros.
+skip.
+apply H;
+[ assumption |
+  exists GT].
+auto.
+(* unbox *)
+econstructor; eauto. skip.
+(* unbox_fetch *)
+destruct HSubst as [GT];
+apply t_unbox_fetch_LF with (Gamma:=Gamma) (G:=G++GT);
+[ skip | apply IHHT; exists GT | transitivity (G' ++ GT) ]; auto;
+transitivity (G & (w, Gamma) ++ GT); [symmetry | ]; auto.
+(* here *)
+constructor; auto. skip.
+(* get_here *)
+destruct HSubst as [GT];
+apply t_get_here_LF with (Gamma:=Gamma) (G:=G++GT);
+[ skip |
+  apply IHHT; exists GT | transitivity (G' ++ GT) ]; auto;
+transitivity (G & (w, Gamma) ++ GT); [symmetry | ]; auto.
+(* letdia *)
+apply t_letdia_LF with (A:=A) (L_t:=L_t)(L_w:=L_w);
+[ skip |
+  apply IHHT; assumption | 
+  intros; apply H]; 
+auto;
+destruct HSubst as [GT];
+exists GT; rew_app; auto.
+(* letdia_get *)
+destruct HSubst as [GT];
+apply t_letdia_get_LF with (A:=A) (Gamma:=Gamma) (G:=G++GT) (L_t:=L_t) (L_w:=L_w);
+[ skip | 
+  apply IHHT; exists GT |
+  intros; apply H | 
+  transitivity (G & (w, Gamma) ++ GT); [ symmetry; auto | transitivity (G0 ++ GT)] ];
+auto; 
+exists GT; rew_app; auto.
+Qed.
+
 Lemma GlobalWeakening:
 forall G G' Ctx Ctx' M A
   (HT: G ++ G' |= Ctx |- M ::: A),
   G & Ctx' ++ G' |= Ctx |- M ::: A.
-Admitted.
+intros; rew_app;
+apply BackgroundSubsetImpl with (G:=G++G'); auto.
+exists (Ctx'::nil); rew_app; symmetry; auto.
+Qed.
+
+Lemma Weakening_general:
+  forall G w Gamma M A
+  (HT: G |= (w, Gamma) |- M ::: A),
+  (forall G' w' Delta Delta',
+    PPermut G (G' & (w', Delta)) ->
+    G' & (w', Delta ++ Delta') |= (w, Gamma) |- M ::: A) /\ 
+  (forall Gamma',
+    G |= (w, Gamma ++ Gamma') |- M ::: A).
+intros;
+remember (w, Gamma) as Ctx;
+generalize dependent Gamma;
+generalize dependent w;
+induction HT; split;
+intros; subst; simpl;
+try (inversion HeqCtx; subst).
+(* hyp *)
+constructor; auto. skip.
+constructor. skip. 
+rewrite Mem_app_or_eq; left; assumption.
+(* lam *)
+apply t_lam_LF with (L:=L). skip. intros; eapply H; eauto.
+apply t_lam_LF with (L:=L). skip. 
+intros; eapply H with (v':=v')  (w:=w0) (Gamma:=(v' ,A)::Gamma0); auto.
+(* appl *)
+econstructor; [skip | eapply IHHT1| eapply IHHT2]; eauto.
+econstructor; [skip | eapply IHHT1| eapply IHHT2]; eauto.
+(* box 1 *)
+apply t_box_LF with (L:=L); intros. skip.
+apply BackgroundSubsetImpl with (G:=G' & (w0, Gamma0) & (w', Delta ++ Delta')).
+  apply H with (w:=w'0) (Gamma:=nil); assumption || eauto.
+  exists (@nil Context_LF); rew_app; auto.
+(* box 2 *)
+apply t_box_LF with (L:=L). skip. 
+intros; eapply H; eauto. 
+(* unbox *)
+constructor. skip. eapply IHHT; eauto.
+constructor. skip. eapply IHHT; eauto.
+(* unbox_fetch 1 *)
+destruct (permut_context_LF_dec (w'0, Delta) (w, Gamma)) as [Eq|Neq]; simpl in *.
+(* = *)
+destruct Eq; subst.
+apply t_unbox_fetch_LF with (G:=G) (Gamma:=Gamma++Delta');
+[ skip |
+  apply IHHT; reflexivity | 
+   ];
+(* FIXME: does this deserve a tactic? *)
+assert (G ~=~ G'0) by
+   (apply PPermut_last_rev with (Gamma := Gamma) (Gamma':= Delta) (w:=w);
+    [ apply permut_sym |
+      transitivity G' ]; auto);
+apply PPermut_last; [ permut_simpl; apply permut_sym  | ]; assumption.
+(* <> *)
+(* FIXME: or this? *)
+assert (exists G0, exists G1, G'0 = G0 & (w, Gamma) ++ G1) by
+  ( apply PPermut_split_neq with (G':=G) (w:=w'0) (Gamma := Delta);
+    [ symmetry; transitivity G' | ]; auto);
+destruct H1 as [GH]; destruct H1 as [GT]; subst G'0.
+apply t_unbox_fetch_LF with (Gamma:=Gamma) (G:=GH ++ GT & (w'0, Delta ++ Delta')).
+skip.
+apply BackgroundSubsetImpl with (G:= (GH ++ GT & (w0, Gamma0)) & (w'0, Delta ++ Delta')).
+  apply IHHT with (w1:=w) (Gamma1:=Gamma) (G':=GH ++ GT & (w0, Gamma0)); auto.
+  (* FIXME: more automation ? *)
+  assert (G ~=~ GH ++ GT & (w'0, Delta)).
+     apply PPermut_last_rev_simpl with (a:=(w, Gamma)).
+     transitivity G'. 
+       auto. 
+       rew_app in *; transitivity (GH ++ (w, Gamma) :: GT & (w'0, Delta)).
+         auto.
+         transitivity (GH ++ GT ++ (w, Gamma) :: (w'0, Delta) :: nil); auto.
+  transitivity ((GH ++ GT & (w'0, Delta)) & (w0, Gamma0));
+  [apply PPermut_last | rew_app]; auto.
+  exists (@ nil Context_LF); rew_app; auto.
+rew_app; transitivity (GH ++ GT ++ (w, Gamma) :: (w'0, Delta++Delta') :: nil);
+[ | symmetry]; auto.
+(* unbox_fetch 2 *)
+apply t_unbox_fetch_LF with (G:=G) (Gamma:=Gamma).
+skip.
+apply IHHT with (w1:=w) (Gamma1:=Gamma); auto.
+auto.
+(* here *)
+constructor. skip. apply IHHT with (w:=w0)(Gamma:=Gamma0); auto. 
+constructor. skip. apply IHHT; auto.
+(* get_here 1 *)
+destruct (permut_context_LF_dec (w', Delta) (w, Gamma)) as [Eq | Neq]; simpl in *.
+(* = *)
+destruct Eq; subst;
+apply t_get_here_LF with (Gamma:=Gamma++Delta') (G:=G).
+skip.
+apply IHHT; auto.
+apply PPermut_last; 
+[ | apply PPermut_last_rev with (w:=w) (Gamma:=Gamma) (Gamma':=Delta)];
+(permut_simpl; apply permut_sym) || transitivity G'; auto.
+(* <> *)
+assert (exists G0, exists G1, G'0 = G0 & (w, Gamma) ++ G1) by
+  ( apply PPermut_split_neq with (G':=G) (w:=w') (Gamma := Delta);
+    [ symmetry; transitivity G' | ]; auto);
+destruct H1 as [GH]; destruct H1 as [GT]; subst G'0.
+apply t_get_here_LF with (Gamma:=Gamma) (G:=GH ++ GT & (w', Delta ++ Delta')).
+skip.
+apply BackgroundSubsetImpl with (G:= (GH ++ GT & (w0, Gamma0)) & (w', Delta ++ Delta')).
+  apply IHHT with (w1:=w) (Gamma1:=Gamma) (G':=GH ++ GT & (w0, Gamma0)); auto.
+  assert (G ~=~ GH ++ GT & (w', Delta)).
+     apply PPermut_last_rev_simpl with (a:=(w, Gamma)).
+     transitivity G'. 
+       auto. 
+       rew_app in *; transitivity (GH ++ (w, Gamma) :: GT & (w', Delta)).
+         auto.
+         transitivity (GH ++ GT ++ (w, Gamma) :: (w', Delta) :: nil); auto.
+  transitivity ((GH ++ GT & (w', Delta)) & (w0, Gamma0));
+  [apply PPermut_last | rew_app]; auto.
+  exists (@ nil Context_LF); rew_app; auto.
+rew_app; transitivity (GH ++ GT ++ (w, Gamma) :: (w', Delta++Delta') :: nil);
+[ | symmetry]; auto.
+(* get_here 2 *)
+apply t_get_here_LF with (G:=G) (Gamma:=Gamma).
+skip.
+apply IHHT with (w1:=w) (Gamma1:=Gamma); auto.
+auto.
+(* letdia *)
+apply t_letdia_LF with (A:=A) (L_w:=L_w) (L_t:=L_t).
+skip.
+apply IHHT with (w:=w0) (Gamma:=Gamma0); auto.
+intros; destruct H with (v':=v') (w':=w'0) (w:=w0) (Gamma:=Gamma0); auto.
+replace ((w'0, (v', A) :: nil) :: G' & (w', Delta ++ Delta')) with
+   (((w'0, (v', A) :: nil) :: G') & (w', Delta ++ Delta')) by
+   (rew_app; reflexivity).
+apply H3; rew_app; auto.
+eapply t_letdia_LF with (A:=A).
+skip.
+apply IHHT; auto.
+intros; eapply H; eauto.
+(* letdia_get 1 *)
+destruct (permut_context_LF_dec (w', Delta) (w, Gamma)) as [Eq | Neq]; simpl in *.
+(* = *)
+destruct Eq; subst;
+apply t_letdia_get_LF with (Gamma:=Gamma++Delta') (G:=G) (A:=A) (L_w:=L_w) (L_t:=L_t).
+skip.
+apply IHHT; auto.
+intros; destruct H with (v':=v') (w':=w') (w1:=w0) (Gamma1:=Gamma0); eauto.
+replace ( (w', (v', A) :: nil) :: G & (w, Gamma ++ Delta') ) with
+  (( (w', (v', A) :: nil) :: G) & (w, Gamma ++ Delta')) by
+  (rew_app; reflexivity).
+eapply H5; auto.
+assert (G ~=~ G').
+  apply PPermut_last_rev with (w:=w) (Gamma:=Gamma) (Gamma':=Delta);
+  [apply permut_sym | transitivity G0]; auto. 
+apply PPermut_last; [permut_simpl; apply permut_sym | ]; auto.
+(* <> *)
+assert (exists G0, exists G1, G' = G0 & (w, Gamma) ++ G1) by 
+  ( apply PPermut_split_neq with (G':=G) (w:=w') (Gamma := Delta);
+    [ symmetry; transitivity G0 | ]; auto);
+destruct H2 as [GH]; destruct H2 as [GT]; subst G'.
+assert (G ~=~ GH ++ GT & (w', Delta)).
+  apply PPermut_last_rev_simpl with (a:=(w, Gamma)).
+  transitivity G0. 
+  auto. 
+  rew_app in *; transitivity (GH ++ (w, Gamma) :: GT & (w', Delta)).
+  auto.
+  transitivity (GH ++ GT ++ (w, Gamma) :: (w', Delta) :: nil); auto.
+apply t_letdia_get_LF with 
+  (Gamma:=Gamma) (G:=GH ++ GT & (w', Delta ++ Delta')) (L_w:=L_w) (L_t:=L_t)(A:=A).
+skip.
+apply BackgroundSubsetImpl with (G:= (GH ++ GT & (w0, Gamma0)) & (w', Delta ++ Delta')).
+apply IHHT with (w1:=w) (Gamma1:=Gamma); auto. 
+  transitivity ((GH ++ GT & (w', Delta)) & (w0, Gamma0));
+  [apply PPermut_last | rew_app]; auto.
+  exists (@ nil Context_LF); rew_app; auto.
+intros; destruct H with (v':=v')(w':=w'0) (w1:=w0) (Gamma1:=Gamma0); auto.
+apply BackgroundSubsetImpl with 
+  (G:=((w'0, (v', A)::nil) :: GH++GT & (w, Gamma)) & (w', Delta ++ Delta')).
+  apply H5.
+  rew_app; constructor; [auto | ].
+  transitivity ((GH ++ GT & (w', Delta)) & (w, Gamma));
+  [apply PPermut_last | rew_app]; auto.
+  exists (@ nil Context_LF); rew_app; auto.
+rew_app.
+transitivity (GH ++ GT ++ (w, Gamma) :: (w', Delta ++ Delta') :: nil); 
+[ | symmetry]; auto.
+(* letdia_get 2 *)
+apply t_letdia_get_LF with (G:=G) (Gamma:=Gamma) (A:=A) (L_w:=L_w)(L_t:=L_t).
+skip.
+apply IHHT with (w1:=w) (Gamma1:=Gamma); auto.
+intros; destruct H with (v':=v')(w':=w') (w1:=w0)(Gamma1:=Gamma0); auto.  
+assumption.
+Qed.
 
 Lemma WeakeningBackgroundElem:
 forall G G' w Delta Delta' Ctx M A
   (HT: G & (w, Delta) ++ G' |= Ctx |- M ::: A),
   G & (w, Delta ++ Delta') ++ G' |= Ctx |- M ::: A.
-Admitted.
+intros;
+apply BackgroundSubsetImpl with (G:=(G++G') & (w, Delta ++ Delta')).
+destruct Ctx; eapply Weakening_general; eauto.
+eexists nil; rew_app; symmetry; auto.
+Qed.
 
 Lemma Weakening:
 forall G w Gamma Gamma' M A
   (HT: G |= (w, Gamma) |- M ::: A),
   G |= (w, Gamma ++ Gamma') |- M ::: A.
-Admitted.
+intros;
+eapply Weakening_general; eassumption.
+Qed.
 
 (* emptyEquiv = map (fun x => (x, nil)) (map fst G) *)
 Fixpoint emptyEquiv (G: Background_LF) : Background_LF :=
@@ -172,10 +439,19 @@ match G with
 | (w, a)::G => (w, nil) :: emptyEquiv G
 end.
 
+(* TODO! *)
 Lemma types_weakened:
 forall G w Gamma M A
+  (Ok: ok_Bg ((w, Gamma)::G))
   (HT: emptyEquiv G |= (w, nil) |- M ::: A),
   G |= (w, Gamma) |- M ::: A.
+Admitted.
+
+(* FIXME: move to lib *)
+Lemma Mem_permut:
+forall A (x:A) G G',
+  G *=* G' ->
+  Mem x G -> Mem x G'.
 Admitted.
 
 Lemma subst_t_preserv_types:
@@ -185,16 +461,15 @@ forall G w Gamma B M N v A
   (HT: G |= (w, Gamma) |- N ::: B), 
   (* "inner" substitution *)
   ( forall Gamma0,
-    (* this should really be permutation... *)
-    Gamma = (v, A) :: Gamma0 ->
+    permut Gamma ((v, A) :: Gamma0) ->
     emptyEquiv G |= (w, nil) |- M ::: A ->
     G |= (w, Gamma0) |- [M // fvar v] N ::: B)
   /\
   (* "outer" substitution *)
   ( forall G0 G' G'' w' Gamma',
-    permut G (G0 & (w', (v,A)::Gamma')) ->
-    permut G' (G0 & (w, Gamma)) ->
-    permut G'' (G0 & (w', Gamma')) ->
+    PPermut G (G0 & (w', (v,A)::Gamma')) ->
+    PPermut G' (G0 & (w, Gamma)) ->
+    PPermut G'' (G0 & (w', Gamma')) ->
     emptyEquiv G' |= (w', nil) |- M ::: A ->
     G'' |= (w, Gamma) |- [M // fvar v] N ::: B).
 intros;
@@ -209,23 +484,23 @@ inversion HeqCtx; subst;
 simpl in *.
 (* hyp *)
 case_if.
-inversion H; subst;
-assert (A = A0) by skip; (* Ok_Bg + HT *)
-subst; apply types_weakened; assumption.
+inversion H1; subst.
+assert (A = A0) by skip. (* Ok_Bg + HT *)
+subst; apply types_weakened. skip. (* ok_Bg *)
+assumption.
 constructor.
 skip. (* ok_Bg *)
-(* Mem part should be automated! *)
-rewrite Mem_cons_eq in HT; destruct HT.
-  inversion H1; subst; elim H; reflexivity.
-  assumption.
-
+apply Mem_permut with (G' := (v0, A0) :: Gamma1) in HT; auto;
+rewrite Mem_cons_eq in HT; destruct HT; auto;
+inversion H2; subst; elim H1; reflexivity.
 case_if.
-inversion H3; subst;
+inversion H3; subst.
 (* v = v0 ->
    Ok_Bg + H + H0 + HT -->
    v0 occurs both in Gamma0 and in G -->
    contradiction *)
 skip.
+
 constructor.
 skip. (* ok_Bg *)
 assumption.
@@ -233,12 +508,12 @@ assumption.
 apply t_lam_LF with (L:=L \u \{v}).
 skip. (* ok_Bg *)
 intros.
-rewrite notin_union in H0; rewrite notin_singleton in H0; destruct H0.
+rewrite notin_union in H2; rewrite notin_singleton in H2; destruct H2.
 unfold open_var in *.
 rewrite <- subst_var_comm.
 eapply H; eauto.
-skip. (* this should really be permutations *)
-intro; elim H2; subst; auto.
+permut_simpl; assumption.
+intro; elim H3; subst; auto.
 auto.
 
 apply t_lam_LF with (L:=L \u \{v}).
@@ -255,80 +530,84 @@ auto.
 econstructor; [ skip | eapply IHHT1 | eapply IHHT2]; eauto.
 econstructor; [ skip | eapply IHHT1 | eapply IHHT2]; eauto.
 (* box *)
-econstructor; [skip | intros].
+apply t_box_LF with (L:=L); [skip | intros].
 unfold open_ctx.
 rewrite <- subst_order_irrelevant_bound.
 eapply H; eauto.
-skip. (* form H1 + weakening + emptyEquiv_last *)
+skip.
 auto.
 
 econstructor; [skip | intros].
 unfold open_ctx.
 rewrite <- subst_order_irrelevant_bound.
 eapply H with (G'' := G'' & (w0, Gamma0)); eauto.
-skip. (* H0 + H2 *)
-skip. (* H3 + H1 + Weakening *)
+skip.
 auto.
 (* unbox *)
 econstructor; [skip | eapply IHHT]; eauto.
 econstructor; [skip | eapply IHHT]; eauto.
 (* unbox_fetch *)
-apply t_unbox_fetch_LF with (G:=G) (Gamma:=Gamma).
+apply t_unbox_fetch_LF with (G:=G) (Gamma:=Gamma); auto.
 skip. (* ok_Bg *)
 eapply IHHT; eauto.
 skip. (* emptyEquiv + permut *)
-assumption.
 
 assert (w <> w0) by skip. (* from Ok_Bg *)
 assert (w <> w'0) by skip. (* Ok_bg + H + H0 *) 
 (* H0 + H + ok_Bg + w <> w'0 -->
    G & (w, Gamma) ~=~ G0 & (w'0, (v, A0) :: Gamma'0) -->
    exists GH, exists GT, G = GH & (w'0, (v,A0)::Gamma'0) ++ GT. *)
-assert (exists GH, exists GT, G = GH & (w'0, (v, A0)::Gamma'0) ++ GT) by skip.
-destruct H6 as (GH, H6); destruct H6 as (GT, H6).
+assert (G & (w, Gamma) ~=~ G0 & (w'0, (v, A0) :: Gamma'0)) by
+  (transitivity G'; auto).
+assert (exists GH, exists GT, G = GH & (w'0, (v, A0)::Gamma'0) ++ GT) by
+  (apply PPermut_split_neq with (w:=w) (Gamma:=Gamma) (G':=G0); auto).
+destruct H7 as (GH, H7); destruct H7 as (GT, H7).
 apply t_unbox_fetch_LF with (G:=GH ++ GT & (w'0, Gamma'0)) (Gamma:=Gamma).
 skip. (* ok_Bg *)
 eapply IHHT with (w1:=w) (Gamma1:=Gamma) (w':=w'0) (Gamma':=Gamma'0)
-                 (G0:=GH ++ GT & (w0, Gamma0)); eauto.
-subst; permut_simpl.
-subst; permut_simpl.
+                 (G0:=GH ++ GT & (w0, Gamma0)); rew_app; auto; subst.
+rew_app; auto.
 skip. (* emptyEquiv + permut *)
-skip. (* H2 + H + H0 *)
+subst; rew_app in *.
+transitivity (G0 & (w'0, Gamma'0)); 
+[ apply PPermut_specialized2 with (Gamma:= (w'0, (v, A0) :: Gamma'0)) | symmetry]; auto.
 (* here *)
 econstructor; [skip | eapply IHHT]; eauto.
 econstructor; [skip | eapply IHHT]; eauto.
 (* get_here *)
-apply t_get_here_LF with (G:=G) (Gamma:=Gamma).
+apply t_get_here_LF with (G:=G) (Gamma:=Gamma); auto.
 skip. (* ok_Bg *)
 eapply IHHT; eauto.
 skip. (* emptyEquiv + permut *)
-assumption.
 
 assert (w <> w0) by skip. (* from Ok_Bg *)
 assert (w <> w') by skip. (* Ok_bg + H + H0 *) 
 (* H0 + H + ok_Bg + w <> w'0 -->
    G & (w, Gamma) ~=~ G0 & (w'0, (v, A0) :: Gamma'0) -->
    exists GH, exists GT, G = GH & (w', (v,A0)::Gamma'0) ++ GT. *)
-assert (exists GH, exists GT, G = GH & (w', (v, A0)::Gamma') ++ GT) by skip.
-destruct H7 as (GH, H7); destruct H7 as (GT, H7).
+assert (G & (w, Gamma) ~=~ G0 & (w', (v, A0) :: Gamma')) by
+  (transitivity G'; auto).
+assert (exists GH, exists GT, G = GH & (w', (v, A0)::Gamma') ++ GT) by
+  (apply PPermut_split_neq with (w:=w) (Gamma:=Gamma) (G':=G0); auto).
+destruct H8 as (GH, H8); destruct H8 as (GT, H8).
 apply t_get_here_LF with (G:=GH ++ GT & (w', Gamma')) (Gamma:=Gamma).
 skip. (* ok_Bg *)
 eapply IHHT with (w1:=w) (Gamma1:=Gamma) (w':=w') (Gamma':=Gamma')
-                 (G0:=GH ++ GT & (w0, Gamma0)); eauto.
-subst; permut_simpl.
-subst; permut_simpl.
+                 (G0:=GH ++ GT & (w0, Gamma0)); rew_app; auto; subst.
+rew_app; auto.
 skip. (* emptyEquiv + permut *)
-skip. (* H2 + H + H0 *)
-
+subst; rew_app in *.
+transitivity (G0 & (w', Gamma')); 
+[ apply PPermut_specialized2 with (Gamma:= (w', (v, A0) :: Gamma')) | symmetry]; auto.
 (* letdia *)
 eapply t_letdia_LF with (L_t := L_t \u \{v}); [skip | eapply IHHT | intros]; eauto.
 unfold open_var in *. unfold open_ctx in *.
-rewrite notin_union in H0; rewrite notin_singleton in H0; destruct H0.
+rewrite notin_union in H2; rewrite notin_singleton in H2; destruct H2.
 rewrite <- subst_order_irrelevant_bound.
 rewrite <- subst_var_comm.
 eapply H; eauto.
 skip. (* weakening + assumption *)
-intro; subst; elim H3; auto.
+intro; subst; elim H4; auto.
 assumption.
 assumption.
 
@@ -338,9 +617,7 @@ rewrite notin_union in H4; rewrite notin_singleton in H4; destruct H4.
 rewrite <- subst_order_irrelevant_bound.
 rewrite <- subst_var_comm.
 eapply H with (G0:=(w'0, (v',A)::nil)::G0) (w'0:=w') (Gamma':=Gamma') (A0:=A0); eauto.
-permut_simpl; auto.
-permut_simpl; auto.
-skip. (* weakening + assumption *)
+skip.
 intro; subst; elim H6; auto.
 assumption.
 assumption.
@@ -350,15 +627,15 @@ assert (w <> w0) by skip. (* from Ok_bg *)
 eapply t_letdia_get_LF with (G:=G) (Gamma:=Gamma) (L_t := L_t \u \{v}); eauto.
 skip. (* ok_Bg *)
 eapply IHHT; eauto.
-skip. (* permut + assumption *)
+skip.
 intros. 
 unfold open_var in *; unfold open_ctx in *.
-rewrite notin_union in H4; rewrite notin_singleton in H4; destruct H4.
+rewrite notin_union in H5; rewrite notin_singleton in H5; destruct H5.
 rewrite <- subst_order_irrelevant_bound.
 rewrite <- subst_var_comm.
 eapply H; eauto.
 skip. (* weakening + permut + assumption *)
-intro; subst; elim H6; auto.
+intro; subst; elim H7; auto.
 auto.
 auto.
 
@@ -369,7 +646,7 @@ subst.
 assert (Gamma = (v, A0) :: Gamma') by skip.
 assert (G1 = G) by skip.
 subst.
-eapply t_letdia_get_LF with (G:=G) (Gamma:=Gamma') (L_t:=L_t \u \{v}); eauto.
+eapply t_letdia_get_LF with (G:=G) (Gamma:=Gamma') (L_t:=L_t \u \{v}); auto.
 skip. (* ok_Bg *)
 eapply IHHT; eauto.
 skip. (* permut + emptyEquiv *)
@@ -379,13 +656,11 @@ rewrite notin_union in H7; rewrite notin_singleton in H7; destruct H7.
 rewrite <- subst_order_irrelevant_bound.
 rewrite <- subst_var_comm.
 eapply H with (G0:=G & (w'0, (v', A)::nil) ) (w'1:=w') (Gamma'0:=Gamma'); eauto.
-permut_simpl.
-permut_simpl.
 skip. (* Weakening + permut + assumption *)
 auto.
 auto.
 auto.
-apply permut_sym; auto.
+symmetry; auto.
 
 (* w <> w' /\
    Ok Bg /\
@@ -393,28 +668,36 @@ apply permut_sym; auto.
    G0 ~=~ (G1 & (w', (v, A0) :: Gamma')) -->
    G & (w, Gamma) ~=~ G1 & (w', (v,A0)::Gamma') -->
    exists GH, exists GT, G1 = GH & (w, Gamma) ++ GT *)
-assert (exists GH, exists GT, G1 = GH & (w, Gamma) ++ GT) by skip.
-destruct H7 as (GH, H7). destruct H7 as (GT, H7).
-eapply t_letdia_get_LF with (G:=GH++GT & (w', Gamma')) (Gamma:=Gamma) (L_t:=L_t \u \{v}).
+assert (G & (w, Gamma) ~=~ G1 & (w', (v, A0) :: Gamma')) by
+  (transitivity G0; auto).
+symmetry in H7.
+assert (exists GH, exists GT, G1 = GH & (w, Gamma) ++ GT) by
+  (apply PPermut_split_neq with (w:=w') (Gamma:=(v,A0) :: Gamma') (G':=G); auto).
+destruct H8 as (GH, H8). destruct H8 as (GT, H8).
+eapply t_letdia_get_LF with (G:=GH++GT & (w', Gamma')) (Gamma:=Gamma) (L_t:=L_t \u \{v}) (L_w:=L_w).
 skip. (* ok_Bg *)
-eapply IHHT with (G0:=GH++GT & (w0,Gamma0)) (Gamma':=Gamma'); eauto.
-permut_simpl. skip. (* H7 + H0 + H1 *)
-permut_simpl.
+eapply IHHT with (w1:=w) (Gamma1:=Gamma) (A0:=A0) (w':=w') (G0:=GH++GT & (w0,Gamma0)) (Gamma':=Gamma'); auto.
+symmetry; subst; rew_app in *; apply PPermut_specialized2 with (Gamma := (w, Gamma)); auto.
+rew_app; auto.
 skip. (* permut + assumption *)
 intros.
 unfold open_var in *; unfold open_ctx in *.
-rewrite notin_union in H8; rewrite notin_singleton in H8; destruct H8.
+rewrite notin_union in H9; rewrite notin_singleton in H9; destruct H9.
 rewrite <- subst_order_irrelevant_bound.
 rewrite <- subst_var_comm.
-eapply H with (G0:=(w'0, (v', A) :: nil) :: (GH ++ GT) & (w, Gamma)) (Gamma':=Gamma'); eauto. 
-subst; permut_simpl. skip. (* H7 + H0 + H1 *)
-permut_simpl.
+eapply H with (v':=v') (w':=w'0) (Gamma1:=Gamma0) (w1:=w0) (A0:=A0) 
+              (v:=v) (G0:=(w'0, (v', A) :: nil) :: (GH ++ GT) & (w, Gamma)) 
+              (w'0:=w') (Gamma':=Gamma'); auto.
+rew_app; constructor; auto;
+symmetry; transitivity (G1 & (w', (v, A0) :: Gamma')); auto;
+subst; rew_app; auto.
+rew_app; constructor; auto.
 skip. (* Weakening + permut + assumption *)
+intro; elim H11; auto.
 auto.
 auto.
-auto.
-skip. (* permut + permut_sym *)
-Admitted. (* No more subgoals but non-instantiated existential variables *)
+symmetry; transitivity (G1 & (w', Gamma')); subst; rew_app in *; auto.
+Qed.
 
 Lemma subst_t_preserv_types_inner:
 forall G w Gamma A B M N v
@@ -431,9 +714,9 @@ Lemma subst_t_preserv_types_outer:
 forall G0 G G' G'' w w' Gamma Gamma' A B M N v
   (H_lc_t: lc_t_LF M)
   (H_lc_w: lc_w_LF M)
-  (G0G: permut G (G0 & (w', (v, A) :: Gamma')))
-  (G0G': permut G' (G0 & (w, Gamma)))
-  (G0G'': permut G'' (G0 & (w', Gamma')))
+  (G0G: PPermut G (G0 & (w', (v, A) :: Gamma')))
+  (G0G': PPermut G' (G0 & (w, Gamma)))
+  (G0G'': PPermut G'' (G0 & (w', Gamma')))
   (HM: emptyEquiv G' |= (w', nil) |- M ::: A)
   (HT: G |= (w, Gamma) |- N ::: B),
   G'' |= (w, Gamma) |- [M // fvar v] N ::: B.
@@ -445,15 +728,15 @@ Lemma rename_w_preserv_types:
 forall G w Gamma A M G' w' Gamma'
   (HT: G |= (w, Gamma) |- M ::: A),
   (* "new" substitution *)
-  ( permut G (G' & (w', Gamma')) ->
+  ( PPermut G (G' & (w', Gamma')) ->
     G' |= (w, Gamma ++ Gamma') |- {{ fctx w // fctx w' }} M ::: A) /\
   (* "old" substitution *)
-  ( permut G (G' & (w', Gamma')) ->
+  ( PPermut G (G' & (w', Gamma')) ->
     G' |= (w', Gamma' ++ Gamma) |- {{ fctx w' // fctx w }} M ::: A) /\
   (* "outer" substitution *)
   (forall G0 w'' Gamma'',
-    permut G (G0 & (w', Gamma') & (w'', Gamma'')) ->
-    permut G' (G0 & (w', Gamma' ++ Gamma'')) ->
+    PPermut G (G0 & (w', Gamma') & (w'', Gamma'')) ->
+    PPermut G' (G0 & (w', Gamma' ++ Gamma'')) ->
     G' |= (w, Gamma) |- {{ fctx w' // fctx w''}} M ::: A).
 intros;
 remember (w, Gamma) as Ctx;
@@ -487,11 +770,10 @@ apply t_lam_LF with (L := L);
 [ skip | (* ok_Bg *)
   intros]; unfold open_var in *;
 rewrite subst_order_irrelevant_free;
-edestruct H; eauto; destruct H3; 
-replace ((v', A) :: Gamma' ++ Gamma0) with (Gamma' ++ (v', A) :: Gamma0)
-  by skip; (* TODO: order of elems in context is irrelevant *)
-eauto;
-apply notin_empty. 
+edestruct H; eauto; destruct H3.
+apply ContextPermutImpl with (Gamma := (Gamma' ++ (v', A) :: Gamma0)); [permut_simpl | ];
+eauto.
+simpl; apply notin_empty. 
 apply t_lam_LF with (L := L);
 [ skip | (* ok_Bg *)
   intros]; unfold open_var in *;
@@ -523,8 +805,7 @@ unfold open_ctx in *;
 rewrite notin_union in H1; destruct H1;
 rewrite notin_singleton in *;
 rewrite <- subst_ctx_comm; auto;
-eapply H; eauto;
-permut_simpl; assumption.
+eapply H; eauto.
 apply t_box_LF with (L:=\{w0} \u L);
 [ skip | (* ok_Bg *)
   intros]; 
@@ -532,8 +813,7 @@ unfold open_ctx in *;
 rewrite notin_union in H1; destruct H1;
 rewrite notin_singleton in *;
 rewrite <- subst_ctx_comm; auto;
-eapply H; eauto;
-permut_simpl; assumption.
+eapply H; eauto.
 apply t_box_LF with (L:=\{w''} \u L);
 [ skip | (* ok_Bg *)
   intros]; 
@@ -541,8 +821,7 @@ unfold open_ctx in *;
 rewrite notin_union in H2; destruct H2;
 rewrite notin_singleton in *;
 rewrite <- subst_ctx_comm; auto;
-eapply H with (G0:=G0 & (w0, Gamma0)) (Gamma':=Gamma') (Gamma'':=Gamma''); eauto;
-permut_simpl; rew_app in *; assumption.
+eapply H with (G0:=G0 & (w0, Gamma0)) (Gamma':=Gamma') (Gamma'':=Gamma''); eauto.
 (* unbox *)
 case_if; 
 (* w0 = w' 
@@ -565,6 +844,7 @@ case_if;
   constructor];
 [ skip | (* ok_Bg *)
   eapply IHHT; eauto].
+
 (* unbox_fetch *)
 case_if.
 (* G' ~=~ G & (w, Gamma)
@@ -573,88 +853,127 @@ case_if.
    w = w'0
    ok_Bg (w, Gamma) :: G -->
    G'0 = G && Gamma'0 = Gamma *)
-assert (Gamma'0 = Gamma) by skip;
-assert (G'0 = G) by skip;
-inversion H1; subst;
-constructor;
-[ skip | (* ok_Bg *)
-  apply IHHT; auto].
+inversion H1; subst.
+assert (Gamma *=* Gamma'0) by skip. (* H + H0 *)
+assert (G ~=~ G'0).
+  apply PPermut_last_rev with (w:=w'0) (Gamma:=Gamma) (Gamma':=Gamma'0);
+  [ | transitivity G']; auto.
+constructor.
+skip.
+apply ContextPermutImpl with (Gamma:=Gamma0 ++ Gamma);
+[ permut_simpl |
+  apply IHHT] ; auto.
+
 (* H: G & (w, Gamma) ~=~ G'
    H0: G' ~=~ G'0 & (w'0, Gamma'0) -->
    G'0 & (w'0, Gamma'0) ~= G & (w, Gamma) 
    H1: w <> w'0 -->
    exists GH, exists GT, G'0 = GH & (w, Gamma) ++ GT *)
-assert (exists GH, exists GT, G'0 = GH & (w, Gamma) ++ GT) as Split by skip;
+assert (G'0 & (w'0, Gamma'0) ~=~ G & (w, Gamma)). symmetry; transitivity G'; auto.
+assert (exists GH, exists GT, G'0 = GH & (w, Gamma) ++ GT) as Split.
+  eapply PPermut_split_neq; eauto; right; intro; subst; elim H1; reflexivity.
 destruct Split as (GH, Split); destruct Split as (GT); subst.
-apply t_unbox_fetch_LF with (G:=GH++GT) (Gamma:=Gamma); 
-[ skip | (* ok_Bg *)
-  eapply IHHT; eauto | ]; 
-permut_simpl;
-(* H + H0 --> G & (w, Gamma) ~=~ GH & (w, Gamma) ++ GT & (w'0, Gamma'0) --> 
-   remove (w,Gamma) from both sides *)
+apply t_unbox_fetch_LF with (G:=GH++GT) (Gamma:=Gamma).
 skip.
+eapply IHHT with (w1:=w) (Gamma1:=Gamma); auto.
+apply PPermut_last_rev_simpl with (a:=(w, Gamma)); rew_app in *; auto.
+rew_app; auto.
 
 case_if.
 (* w = w0 --> ok_Bg w,.. :: G & (w0, .. ) --> contradiction *)
 skip.
 destruct (eq_var_dec w w'0).
 (* w = w'0 follows that G = G'0 and Gamma = Gamma'0 *)
-assert (Gamma'0 = Gamma) by skip;
-assert (G'0 = G) by skip;
-subst; constructor; [skip | ].
-eapply IHHT with (w:=w'0) (Gamma1:=Gamma) (Gamma':=Gamma0); eauto.
+subst.
+assert (Gamma *=* Gamma'0) by skip. (* H + H0 *)
+assert (G ~=~ G'0).
+  apply PPermut_last_rev with (w:=w'0) (Gamma:=Gamma) (Gamma':=Gamma'0);
+  [ | transitivity G']; auto.
+subst; constructor.
+skip.
+apply ContextPermutImpl with (Gamma:=Gamma ++ Gamma0);
+[ permut_simpl |
+  eapply IHHT with (w:=w'0) (Gamma1:=Gamma) (Gamma':=Gamma0)] ; auto.
+
 (* w <> w'0
    H & H0 -> G'0 & (w'0, Gamma'0) ~=~ G & (w, Gamma) -->
    exists GH, exists GT, G'0 = GH & (w, Gamma) ++ GT *)
-assert (exists GH, exists GT, G'0 = GH & (w, Gamma) ++ GT) as Split by skip;
+assert (G'0 & (w'0, Gamma'0) ~=~ G & (w, Gamma)). symmetry; transitivity G'; auto.
+assert (exists GH, exists GT, G'0 = GH & (w, Gamma) ++ GT) as Split.
+  eapply PPermut_split_neq; eauto; right; intro; subst; elim H1; reflexivity.
 destruct Split as (GH, Split); destruct Split as (GT); subst.
-apply t_unbox_fetch_LF with (G:=GH++GT) (Gamma:=Gamma);
-[ skip | (* ok_Bg *)
-  eapply IHHT; eauto | ];
-permut_simpl.
-(* H + H0 --> G & (w, Gamma) ~=~ GH & (w, Gamma) ++ GT & (w'0, Gamma'0) --> 
-   remove (w,Gamma) from both sides *)
+apply t_unbox_fetch_LF with (G:=GH++GT) (Gamma:=Gamma).
 skip.
+eapply IHHT; auto.
+apply PPermut_last_rev_simpl with (a:=(w, Gamma)); rew_app in *.
+transitivity (GH ++ GT ++ (w0, Gamma0) :: (w'0, Gamma'0) :: (w, Gamma) :: nil); auto.
+rew_app; auto.
 
 case_if.
 (* w = w'' 
    (G0 & (w'0, Gamma'0) & (w'', Gamma'')) ~=~ G & (w, Gamma) -->
    G0 & (w'0, Gamma'0) ~=~ G /\ Gamma'' = Gamma *)
-inversion H2;
-assert (permut G (G0 & (w'0, Gamma'0))) by skip;
-assert (Gamma'' = Gamma) by skip;
-subst.
-apply t_unbox_fetch_LF with (G:=G0) (Gamma:=Gamma'0 ++ Gamma).
+inversion H2; subst.
+assert (Gamma *=* Gamma'') by skip. (* H + H0 *)
+assert (G ~=~ G0 & (w'0, Gamma'0)).
+  apply PPermut_last_rev with (w:=w'') (Gamma:=Gamma) (Gamma':=Gamma'');
+  [ | transitivity G']; auto.
+apply t_unbox_fetch_LF with (G:=G0) (Gamma := Gamma'0 ++ Gamma).
 skip. (* ok_Bg *)
-apply IHHT; eauto.
-(* TODO: get rid of those 2 proofs, some permut_auto .. *)
-permut_simpl; assumption.
-apply permut_sym; assumption.
-assert (w <> w0) by skip. (* from ok_Bg *)
+apply IHHT; auto.
+transitivity (G0 & (w'0, Gamma'0) & (w0, Gamma0)); auto.
+symmetry; transitivity (G0 & (w'0, Gamma'0 ++ Gamma'')); auto.
+apply PPermut_last;
+[ permut_simpl; apply permut_sym | ]; auto.
+
 destruct (eq_var_dec w w'0).
-(* w = w'0 follows that G = G'0 and Gamma = Gamma'0 *)
-assert (Gamma'0 = Gamma) by skip;
-assert (G'0 = G) by skip;
-subst. 
-(* ok_Bg w'0, Gamma :: G & (w0, Gamma0)
-   G ~=~ G0 & (w'0, Gamma ++ Gamma'') --->
-   variables from Gamma will be doubled; they should be unique;
-   contradiction *)
-skip.
+(* w = w'0*)
+subst.
+assert (Gamma *=* Gamma'0) by skip. (* H + H0 *)
+assert (G ~=~ G0 & (w'', Gamma'')).
+  apply PPermut_last_rev with (w:=w'0) (Gamma:=Gamma) (Gamma':=Gamma'0);
+  [ | transitivity G']; auto.   
+  transitivity (G0 & (w'0, Gamma'0) & (w'', Gamma'')); auto.
+apply t_unbox_fetch_LF with (G:=G0) (Gamma := Gamma ++ Gamma'').
+skip. (* ok_Bg *)
+eapply IHHT with (G':=G0 & (w0, Gamma0)) (Gamma' := Gamma''); auto.
+transitivity (G0 & (w'', Gamma'') & (w0, Gamma0)); auto.
+symmetry; transitivity (G0 & (w'0, Gamma'0 ++ Gamma'')); auto.
+apply PPermut_last;
+[ permut_simpl; apply permut_sym | ]; auto.
+
 (* w <> w'0 /\ w <> w'
    H & H0 -> G0 & (w'0, Gamma'0) & (w'', Gamma'') ~=~ G & (w, Gamma) -->
    exists GH, exists GT, G0 = GH & (w, Gamma) ++ GT *)
-assert (exists GH, exists GT, G0 = GH & (w, Gamma) ++ GT) as Split by skip;
-destruct Split as (GH, Split); destruct Split as (GT); subst.
+assert (G0 & (w'0, Gamma'0) & (w'', Gamma'')  ~=~ G & (w, Gamma)). symmetry; transitivity G'; auto.
+assert (exists GH, exists GT, G0 & (w'0, Gamma'0) = GH & (w, Gamma) ++ GT) as Split.
+  apply PPermut_split_neq with (w:=w'') (Gamma:=Gamma'') (G':= G); eauto.
+  right; intro; subst; elim H2; auto.
+assert (exists GH, exists GT, G0 = GH & (w, Gamma) ++ GT) as Split'.
+  destruct Split as (GH, Split); destruct Split as (GT).
+  apply PPermut_split_neq with (w:=w'0) (Gamma:=Gamma'0) (G':=GH ++ GT).
+  rew_app; transitivity (GH & (w, Gamma) ++ GT); 
+    [ rewrite H4 | rewrite <- app_last; symmetry]; auto.
+  right; intro; subst; elim n; reflexivity.
+destruct Split' as (GH, Split'); destruct Split' as (GT).
 apply t_unbox_fetch_LF with (G:=GH++GT & (w'0, Gamma'0++Gamma'')) (Gamma:=Gamma).
 skip.
-eapply IHHT with (w1:=w) (Gamma1:=Gamma) (G0:=GH++GT & (w0,Gamma0)) (Gamma':=Gamma'0) (Gamma'':=Gamma''); eauto.
-(* permut_auto desperately needed! *)
-permut_simpl; skip. (* H + H1 + permutation magic *)
-permut_simpl.
-apply permut_sym.
-apply permut_trans with (l2 := (GH & (w, Gamma) ++ GT) & (w'0, Gamma'0 ++ Gamma''));
-[auto | permut_simpl].
+eapply IHHT with (w1:=w) (Gamma1:=Gamma) (G0:=GH++GT & (w0,Gamma0)) (Gamma':=Gamma'0) (Gamma'':=Gamma''); auto.
+
+assert (G & (w, Gamma) ~=~ G0 & (w'0, Gamma'0) & (w'', Gamma'')) by (transitivity G'; auto).
+subst; rew_app in *.
+assert (G & (w, Gamma) ~=~ 
+       (GH ++ GT ++ (w'0, Gamma'0) :: (w'', Gamma'') :: nil) &  (w, Gamma)).
+transitivity (GH ++ (w, Gamma) :: GT ++  (w'0, Gamma'0) :: (w'', Gamma'') :: nil); auto.
+transitivity ((GH ++ GT ++ (w'0, Gamma'0) :: (w'', Gamma'') :: nil) & (w0, Gamma0)).
+apply PPermut_last; auto.
+apply PPermut_last_rev_simpl with (a:=(w, Gamma)); auto.
+rew_app; auto.
+rew_app; auto.
+rew_app; symmetry. 
+transitivity (G0 & (w'0, Gamma'0 ++ Gamma'')); auto.
+subst; rew_app; auto.
+
 (* here  -- same as unbox *)
 case_if; 
 (* w0 = w' 
@@ -678,96 +997,135 @@ case_if;
 [ skip | (* ok_Bg *)
   eapply IHHT; eauto].
 
-(* get_here  -- same as unbox_fetch *)
+(* get_here *)
 case_if.
 (* G' ~=~ G & (w, Gamma)
-   G' ~=~ G'0 & (w', Gamma') -->
-   G'0 & (w', Gamma') ~= G & (w, Gamma) 
-   w = w'
+   G' ~=~ G'0 & (w'0, Gamma'0) -->
+   G'0 & (w'0, Gamma'0) ~= G & (w, Gamma) 
+   w = w'0
    ok_Bg (w, Gamma) :: G -->
-   G'0 = G && Gamma' = Gamma *)
-assert (Gamma' = Gamma) by skip;
-assert (G'0 = G) by skip;
-inversion H2; subst;
-constructor;
-[ skip | (* ok_Bg *)
-  apply IHHT; auto].
-(* H: G & (w, Gamma) ~=~ G'
-   H0: G' ~=~ G'0 & (w', Gamma') -->
-   G'0 & (w', Gamma') ~= G & (w, Gamma) 
-   H1: w <> w' -->
-   exists GH, exists GT, G'0 = GH & (w, Gamma) ++ GT *)
-assert (exists GH, exists GT, G'0 = GH & (w, Gamma) ++ GT) as Split by skip;
-destruct Split as (GH, Split); destruct Split as (GT); subst.
-apply t_get_here_LF with (G:=GH++GT) (Gamma:=Gamma); 
-[ skip | (* ok_Bg *)
-  eapply IHHT; eauto | ]; 
-permut_simpl;
-(* H + H0 --> G & (w, Gamma) ~=~ GH & (w, Gamma) ++ GT & (w'0, Gamma'0) --> 
-   remove (w,Gamma) from both sides *)
+   G'0 = G && Gamma'0 = Gamma *)
+inversion H2; subst.
+assert (Gamma *=* Gamma') by skip. (* H + H0 *)
+assert (G ~=~ G'0).
+  apply PPermut_last_rev with (w:=w') (Gamma:=Gamma) (Gamma':=Gamma');
+  [ | transitivity G']; auto.
+constructor.
 skip.
+apply ContextPermutImpl with (Gamma:=Gamma0 ++ Gamma);
+[ permut_simpl |
+  apply IHHT] ; auto.
+
+(* H: G & (w, Gamma) ~=~ G'
+   H0: G' ~=~ G'0 & (w'0, Gamma'0) -->
+   G'0 & (w'0, Gamma'0) ~= G & (w, Gamma) 
+   H1: w <> w'0 -->
+   exists GH, exists GT, G'0 = GH & (w, Gamma) ++ GT *)
+assert (G'0 & (w', Gamma') ~=~ G & (w, Gamma)). symmetry; transitivity G'; auto.
+assert (exists GH, exists GT, G'0 = GH & (w, Gamma) ++ GT) as Split.
+  eapply PPermut_split_neq; eauto; right; intro; subst; elim H2; reflexivity.
+destruct Split as (GH, Split); destruct Split as (GT); subst.
+apply t_get_here_LF with (G:=GH++GT) (Gamma:=Gamma).
+skip.
+eapply IHHT with (w1:=w) (Gamma1:=Gamma); auto.
+apply PPermut_last_rev_simpl with (a:=(w, Gamma)); rew_app in *; auto.
+rew_app; auto.
 
 case_if.
 (* w = w0 --> ok_Bg w,.. :: G & (w0, .. ) --> contradiction *)
 skip.
 destruct (eq_var_dec w w').
-(* w = w'0 follows that G = G'0 and Gamma = Gamma' *)
-assert (Gamma' = Gamma) by skip;
-assert (G'0 = G) by skip;
-subst; constructor; [skip | ].
-eapply IHHT with (w:=w') (Gamma1:=Gamma) (Gamma':=Gamma0); eauto.
+(* w = w'0 follows that G = G'0 and Gamma = Gamma'0 *)
+subst.
+assert (Gamma *=* Gamma') by skip. (* H + H0 *)
+assert (G ~=~ G'0).
+  apply PPermut_last_rev with (w:=w') (Gamma:=Gamma) (Gamma':=Gamma');
+  [ | transitivity G']; auto.
+subst; constructor.
+skip.
+apply ContextPermutImpl with (Gamma:=Gamma ++ Gamma0);
+[ permut_simpl |
+  eapply IHHT with (w:=w') (Gamma1:=Gamma) (Gamma':=Gamma0)] ; auto.
+
 (* w <> w'0
    H & H0 -> G'0 & (w'0, Gamma'0) ~=~ G & (w, Gamma) -->
    exists GH, exists GT, G'0 = GH & (w, Gamma) ++ GT *)
-assert (exists GH, exists GT, G'0 = GH & (w, Gamma) ++ GT) as Split by skip;
+assert (G'0 & (w', Gamma') ~=~ G & (w, Gamma)). symmetry; transitivity G'; auto.
+assert (exists GH, exists GT, G'0 = GH & (w, Gamma) ++ GT) as Split.
+  eapply PPermut_split_neq; eauto; right; intro; subst; elim H1; reflexivity.
 destruct Split as (GH, Split); destruct Split as (GT); subst.
-apply t_get_here_LF with (G:=GH++GT) (Gamma:=Gamma);
-[ skip | (* ok_Bg *)
-  eapply IHHT; eauto | ];
-permut_simpl.
-(* H + H0 --> G & (w, Gamma) ~=~ GH & (w, Gamma) ++ GT & (w'0, Gamma'0) --> 
-   remove (w,Gamma) from both sides *)
+apply t_get_here_LF with (G:=GH++GT) (Gamma:=Gamma).
 skip.
+eapply IHHT; auto.
+apply PPermut_last_rev_simpl with (a:=(w, Gamma)); rew_app in *.
+transitivity (GH ++ GT ++ (w0, Gamma0) :: (w', Gamma') :: (w, Gamma) :: nil); auto.
+rew_app; auto.
 
 case_if.
 (* w = w'' 
    (G0 & (w'0, Gamma'0) & (w'', Gamma'')) ~=~ G & (w, Gamma) -->
    G0 & (w'0, Gamma'0) ~=~ G /\ Gamma'' = Gamma *)
-inversion H3;
-assert (permut G (G0 & (w', Gamma'))) by skip;
-assert (Gamma'' = Gamma) by skip;
-subst.
-apply t_get_here_LF with (G:=G0) (Gamma:=Gamma' ++ Gamma).
+inversion H3; subst.
+assert (Gamma *=* Gamma'') by skip. (* H + H0 *)
+assert (G ~=~ G0 & (w', Gamma')).
+  apply PPermut_last_rev with (w:=w'') (Gamma:=Gamma) (Gamma':=Gamma'');
+  [ | transitivity G']; auto.
+apply t_get_here_LF with (G:=G0) (Gamma := Gamma' ++ Gamma).
 skip. (* ok_Bg *)
-apply IHHT; eauto.
-(* TODO: get rid of those 2 proofs, some permut_auto .. *)
-permut_simpl; assumption.
-apply permut_sym; assumption.
-assert (w <> w0) by skip. (* from ok_Bg *)
+apply IHHT; auto.
+transitivity (G0 & (w', Gamma') & (w0, Gamma0)); auto.
+symmetry; transitivity (G0 & (w', Gamma' ++ Gamma'')); auto.
+apply PPermut_last;
+[ permut_simpl; apply permut_sym | ]; auto.
+
 destruct (eq_var_dec w w').
-(* w = w'0 follows that G = G'0 and Gamma = Gamma'0 *)
-assert (Gamma' = Gamma) by skip;
-assert (G'0 = G) by skip;
-subst. 
-(* ok_Bg w'0, Gamma :: G & (w0, Gamma0)
-   G ~=~ G0 & (w'0, Gamma ++ Gamma'') --->
-   variables from Gamma will be doubled; they should be unique;
-   contradiction *)
-skip.
+(* w = w'0*)
+subst.
+assert (Gamma *=* Gamma') by skip. (* H + H0 *)
+assert (G ~=~ G0 & (w'', Gamma'')).
+  apply PPermut_last_rev with (w:=w') (Gamma:=Gamma) (Gamma':=Gamma');
+  [ | transitivity G']; auto.   
+  transitivity (G0 & (w', Gamma') & (w'', Gamma'')); auto.
+apply t_get_here_LF with (G:=G0) (Gamma := Gamma ++ Gamma'').
+skip. (* ok_Bg *)
+eapply IHHT with (G':=G0 & (w0, Gamma0)) (Gamma' := Gamma''); auto.
+transitivity (G0 & (w'', Gamma'') & (w0, Gamma0)); auto.
+symmetry; transitivity (G0 & (w', Gamma' ++ Gamma'')); auto.
+apply PPermut_last;
+[ permut_simpl; apply permut_sym | ]; auto.
+
 (* w <> w'0 /\ w <> w'
    H & H0 -> G0 & (w'0, Gamma'0) & (w'', Gamma'') ~=~ G & (w, Gamma) -->
    exists GH, exists GT, G0 = GH & (w, Gamma) ++ GT *)
-assert (exists GH, exists GT, G0 = GH & (w, Gamma) ++ GT) as Split by skip;
-destruct Split as (GH, Split); destruct Split as (GT); subst.
+assert (G0 & (w', Gamma') & (w'', Gamma'')  ~=~ G & (w, Gamma)). symmetry; transitivity G'; auto.
+assert (exists GH, exists GT, G0 & (w', Gamma') = GH & (w, Gamma) ++ GT) as Split.
+  apply PPermut_split_neq with (w:=w'') (Gamma:=Gamma'') (G':= G); eauto.
+  right; intro; subst; elim H2; auto.
+assert (exists GH, exists GT, G0 = GH & (w, Gamma) ++ GT) as Split'.
+  destruct Split as (GH, Split); destruct Split as (GT).
+  apply PPermut_split_neq with (w:=w') (Gamma:=Gamma') (G':=GH ++ GT).
+  rew_app; transitivity (GH & (w, Gamma) ++ GT); 
+    [ rewrite H5 | rewrite <- app_last; symmetry]; auto.
+  right; intro; subst; elim n; reflexivity.
+destruct Split' as (GH, Split'); destruct Split' as (GT).
 apply t_get_here_LF with (G:=GH++GT & (w', Gamma'++Gamma'')) (Gamma:=Gamma).
 skip.
-eapply IHHT with (w1:=w) (Gamma1:=Gamma) (G0:=GH++GT & (w0,Gamma0)) (Gamma':=Gamma') (Gamma'':=Gamma''); eauto.
-(* permut_auto desperately needed! *)
-permut_simpl; skip. (* H + H1 + permutation magic *)
-permut_simpl.
-apply permut_sym.
-apply permut_trans with (l2 := (GH & (w, Gamma) ++ GT) & (w', Gamma' ++ Gamma''));
-[auto | permut_simpl].
+eapply IHHT with (w1:=w) (Gamma1:=Gamma) (G0:=GH++GT & (w0,Gamma0)) (Gamma':=Gamma') (Gamma'':=Gamma''); auto.
+
+assert (G & (w, Gamma) ~=~ G0 & (w', Gamma') & (w'', Gamma'')) by (transitivity G'; auto).
+subst; rew_app in *.
+assert (G & (w, Gamma) ~=~ 
+       (GH ++ GT ++ (w', Gamma') :: (w'', Gamma'') :: nil) &  (w, Gamma)).
+transitivity (GH ++ (w, Gamma) :: GT ++  (w', Gamma') :: (w'', Gamma'') :: nil); auto.
+transitivity ((GH ++ GT ++ (w', Gamma') :: (w'', Gamma'') :: nil) & (w0, Gamma0)).
+apply PPermut_last; auto.
+apply PPermut_last_rev_simpl with (a:=(w, Gamma)); auto.
+rew_app; auto.
+rew_app; auto.
+rew_app; symmetry. 
+transitivity (G0 & (w', Gamma' ++ Gamma'')); auto.
+subst; rew_app; auto.
+
 (* letdia *)
 case_if.
 (* w0 = w' ->
@@ -784,7 +1142,6 @@ unfold open_var in *; unfold open_ctx in *.
 rewrite <- subst_ctx_comm.
 rewrite subst_order_irrelevant_free.
 eapply H with (w:=w0) (Gamma:=Gamma0) (w':=w'0); eauto.
-permut_simpl; assumption.
 simpl; auto.
 intro; subst; elim H4; reflexivity.
 
@@ -799,7 +1156,6 @@ unfold open_var in *; unfold open_ctx in *.
 rewrite <- subst_ctx_comm.
 rewrite subst_order_irrelevant_free.
 eapply H with (w:=w0) (Gamma:=Gamma0) (w':=w'0); eauto.
-permut_simpl; assumption.
 simpl; auto.
 intro; subst; elim H4; reflexivity.
 
@@ -816,54 +1172,69 @@ unfold open_var in *; unfold open_ctx in *.
 rewrite <- subst_ctx_comm.
 rewrite subst_order_irrelevant_free.
 eapply H with (w:=w0) (Gamma:=Gamma0) (G0:=G0 & ((w'0, (v', A)::nil))); eauto.
-permut_simpl; rew_app in *; eassumption.
-permut_simpl; assumption.
 simpl; auto.
 intro; subst; elim H5; reflexivity.
+
 (* letdia_get *)
 case_if.
 inversion H3; subst.
 (* w = w' ->
    H1 + H0 = G & w', Gamma ~=~ G' & w', Gamma' ->
    Gamma = Gamma' /\ G = G' *)
-assert (Gamma=Gamma') by skip;
-assert (G = G') by skip;
-subst.   
+assert (Gamma *=* Gamma') by skip.
+assert (G ~=~ G').
+  apply PPermut_last_rev with (w:=w') (Gamma:=Gamma) (Gamma':=Gamma');
+  [ | transitivity G0]; auto.
 eapply t_letdia_LF with (L_w := L_w \u \{w'}).
 skip. (* ok_Bg *)
-eapply IHHT; eauto.
+apply ContextPermutImpl with (Gamma := Gamma0++Gamma); [permut_simpl|]; auto.
+eapply IHHT; auto.
 intros. 
-rewrite notin_union in H5; destruct H5.
-rewrite notin_singleton in H6.
+rewrite notin_union in H7; destruct H7.
+rewrite notin_singleton in H8.
 unfold open_var in *; unfold open_ctx in *.
 rewrite <- subst_ctx_comm.
 rewrite subst_order_irrelevant_free.
-eapply H with (w:=w0) (Gamma:=Gamma0); eauto.
+eapply H with (v':=v') (w'0:=w'0) (w:=w0); auto. eauto.
+rew_app; auto.
 simpl; auto.
-intro; subst; elim H6; reflexivity.
+intro; subst; elim H8; reflexivity.
 
 destruct (eq_var_dec w w0).
 subst; skip. (* ok_Bg -> contradiction *)
 (* H0 + H1: G & (w, Gamma) ~=~ G' & (w', Gamma') -->
    exists GH, exists GT, G = GH & (w', Gamma') ++ GT *)
-assert (exists GH, exists GT, G' = GH & (w, Gamma) ++ GT) by skip;
-destruct H4 as (GH, H4); destruct H4 as (GT, H4).
+assert (G' & (w', Gamma') ~=~ G & (w, Gamma)). symmetry; transitivity G0; auto.
+assert (exists GH, exists GT, G' = GH & (w, Gamma) ++ GT).
+  eapply PPermut_split_neq; eauto. right; intro; subst. elim H3; reflexivity.
+destruct H5 as (GH, H5); destruct H5 as (GT, H5).
+assert (G & (w, Gamma) ~=~ 
+       (GH ++ GT ++ (w', Gamma') :: nil) &  (w, Gamma));
+[subst; symmetry | rew_app]; auto.
+apply PPermut_last; auto;
+apply PPermut_last_rev_simpl with (a:=(w, Gamma)); auto;
+transitivity ((GH & (w, Gamma) ++ GT) & (w', Gamma'));
+[rew_app in *; symmetry | ]; auto.
 apply t_letdia_get_LF with (L_w:=L_w \u \{w'}) (L_t:=L_t) (A:=A) (G:=GH++GT) (Gamma:=Gamma).
 skip. (* ok_Bg *)
 eapply IHHT with (w1:=w) (G0:=GH++GT) (w':=w0) (Gamma':=Gamma0) (Gamma'':=Gamma');
-eauto.
-subst; permut_simpl. skip. (* H0 + H1 *)
+auto.
+transitivity ((GH ++ GT & (w', Gamma')) & (w0, Gamma0)).
+apply PPermut_last; auto.
+apply PPermut_last_rev_simpl with (a:=(w, Gamma)); auto.
+rew_app; auto.
 intros. 
-rewrite notin_union in H6; destruct H6.
-rewrite notin_singleton in H7.
+rewrite notin_union in H8; destruct H8.
+rewrite notin_singleton in H9.
 unfold open_var in *; unfold open_ctx in *.
 rewrite <- subst_ctx_comm.
 rewrite subst_order_irrelevant_free.
-eapply H with (w1:=w0) (Gamma1:=Gamma0); eauto.
-permut_simpl. skip. (* H0 + H1 *)
+eapply H with (w1:=w0) (Gamma1:=Gamma0); auto.
+rew_app; constructor; auto.
+transitivity ((GH ++ GT & (w', Gamma')) & (w, Gamma)); [ | rew_app]; auto.
 simpl; auto.
-intro; subst; elim H7; auto.
-subst; permut_simpl.
+intro; subst; elim H9; auto.
+subst; rew_app; auto.
 
 case_if.
 skip. (* w = w0 --> ok_Bg gives contradiction *)
@@ -871,99 +1242,124 @@ destruct (eq_var_dec w w').
 subst; skip. (* H0 + Ok_Bg gives contradiction *) 
 (* H0 + H1: G & (w, Gamma) ~=~ G' & (w', Gamma') -->
    exists GH, exists GT, G = GH & (w', Gamma') ++ GT *)
-assert (exists GH, exists GT, G' = GH & (w, Gamma) ++ GT) by skip;
-destruct H4 as (GH, H4); destruct H4 as (GT, H4).
+assert (G' & (w', Gamma') ~=~ G & (w, Gamma)). symmetry; transitivity G0; auto.
+assert (exists GH, exists GT, G' = GH & (w, Gamma) ++ GT).
+  eapply PPermut_split_neq; eauto. 
+destruct H5 as (GH, H5); destruct H5 as (GT, H5).
 apply t_letdia_get_LF with (L_w:=L_w \u \{w0}) (L_t:=L_t) (A:=A) (G:=GH++GT) (Gamma:=Gamma).
 skip. (* ok_Bg *)
-eapply IHHT; eauto.
-subst; permut_simpl. skip. (* H0 + H1 *)
+eapply IHHT; auto.
+apply PPermut_last; auto; apply PPermut_last_rev_simpl with (a:=(w, Gamma)).
+transitivity (GH & (w, Gamma) ++ GT & (w', Gamma')); [ | rew_app]; auto.
+subst; symmetry; rew_app in *; auto.
 intros. 
-rewrite notin_union in H6; destruct H6.
-rewrite notin_singleton in H7.
+rewrite notin_union in H7; destruct H7.
+rewrite notin_singleton in H8.
 unfold open_var in *; unfold open_ctx in *.
 rewrite <- subst_ctx_comm.
 rewrite subst_order_irrelevant_free.
-eapply H with (w1:=w0) (Gamma1:=Gamma0); eauto.
-permut_simpl. skip. (* H0 + H1 + H4 *)
+eapply H with (w1:=w0) (Gamma1:=Gamma0); auto.
+rew_app; constructor; auto.
+subst; rew_app in *; symmetry.
+transitivity ( GH ++ (w, Gamma) :: GT & (w', Gamma')); auto.
 simpl; auto.
-intro; subst; elim H7; auto.
-subst; permut_simpl.
+intro; subst; elim H8; auto.
+subst; symmetry; auto.
 
 case_if.
 inversion H4; subst.
 (* H0 + H1 + Ok_Bg --> Gamma'' = Gamma & G0 & (w', Gamma') ~=~ G *)
-assert (Gamma'' = Gamma) by skip.
-assert (G1 & (w', Gamma') = G) by skip.
-subst.
+assert (Gamma *=* Gamma'') by skip.
+assert (G1 & (w', Gamma') ~=~ G).
+  apply PPermut_last_rev with (w:=w'') (Gamma:=Gamma'') (Gamma':=Gamma);
+  [ | transitivity G0]; auto. apply permut_sym; auto. symmetry; auto.
+  symmetry; auto.  
 eapply t_letdia_get_LF with (G:=G1) (Gamma:=Gamma'++Gamma) (L_w:=L_w \u \{w''}).
 skip.
-eapply IHHT; eauto. 
-permut_simpl.
+eapply IHHT with (Gamma':=Gamma'); auto. 
+symmetry; auto.
 intros. 
 unfold open_var in *; unfold open_ctx in *.
 rewrite <- subst_ctx_comm.
 rewrite subst_order_irrelevant_free.
-eapply H with (w:=w0) (G0:=(w'0, (v',A)::nil)::G1); eauto. 
-permut_simpl.
-permut_simpl.
+eapply H with (w:=w0) (G0:=(w'0, (v',A)::nil)::G1) (Gamma':=Gamma') (Gamma'':=Gamma); auto. eauto. 
+rew_app; constructor; [ | symmetry]; auto.
+rewrite <- H6; rew_app; auto.
 simpl; auto.
-rewrite notin_union in H6; 
-rewrite notin_singleton in H6;
-destruct H6; intro; elim H7; auto.
-apply permut_sym; auto.
+rewrite notin_union in H8; 
+rewrite notin_singleton in H8;
+destruct H8; intro; elim H9; auto.
+symmetry; transitivity (G1 & (w', Gamma' ++ Gamma'')); auto.
+apply PPermut_last; auto; permut_simpl; apply permut_sym; auto.
 
 destruct (eq_var_dec w w').
 subst.
 (* H0 + H1 + Ok_Bg --> Gamma = Gamma' /\ G0 & (w'',Gamma'') = G *)
-assert (Gamma' = Gamma) by skip.
-assert (G1 & (w'', Gamma'') = G) by skip.
-subst.
-eapply t_letdia_get_LF with (G:=G1) (Gamma:=Gamma++Gamma'') (L_w:=L_w \u \{w''}).
+assert (Gamma *=* Gamma') by skip.
+assert (G1 & (w'', Gamma'') ~=~ G).
+  apply PPermut_last_rev with (w:=w') (Gamma:=Gamma') (Gamma':=Gamma);
+  [ | transitivity G0]; auto. apply permut_sym; auto. symmetry; auto.
+  transitivity (G1 & (w', Gamma') & (w'', Gamma'')); auto.
+  symmetry; auto.  
+eapply t_letdia_get_LF with (G:=G1) (Gamma:=Gamma++Gamma'') (L_w:=L_w \u \{w''}) (L_t := L_t).
 skip.
-eapply IHHT with (w:=w'); eauto. 
-permut_simpl.
+eapply IHHT with (w:=w'); auto. 
+transitivity ((G1 & (w'', Gamma'')) & (w0, Gamma0)). 
+  apply PPermut_last; [ | symmetry]; auto.
+  auto.
 intros. 
 unfold open_var in *; unfold open_ctx in *.
 rewrite <- subst_ctx_comm.
 rewrite subst_order_irrelevant_free.
-eapply H with (w:=w0) (G0:=(w'0, (v',A)::nil)::G1) (Gamma':=Gamma); eauto. 
-permut_simpl.
-permut_simpl.
+eapply H with (w:=w0) (G0:=(w'0, (v',A)::nil)::G1) (Gamma':=Gamma) (Gamma'':=Gamma''); auto.rew_app; constructor; auto.
+symmetry; transitivity ((G1 ++ (w'', Gamma'')::nil) & (w', Gamma)); auto.
+rew_app; auto. 
 simpl; auto.
-rewrite notin_union in H6; 
-rewrite notin_singleton in H6;
-destruct H6; intro; elim H7; auto.
-apply permut_sym; auto.
+rewrite notin_union in H8; 
+rewrite notin_singleton in H8.
+destruct H8. intro. elim H9; eauto.
+symmetry; transitivity (G1 & (w', Gamma' ++ Gamma'')); auto.
+apply PPermut_last; auto; permut_simpl; apply permut_sym; auto.
+
 (* H0 + H1: G & (w, Gamma) ~=~ G1 & (w', Gamma') & (w'', Gamma'') -->
    exists GH, exists GT, G1 = GH & (w, Gamma) & (w', Gamma') ++ GT *)
-assert (exists GH, exists GT, G1 = GH & (w, Gamma) ++ GT) by skip;
-destruct H5 as (GH, H5); destruct H5 as (GT, H5); subst.
+assert (G & (w, Gamma) ~=~ G1 & (w', Gamma') & (w'', Gamma'')). symmetry; transitivity G0; symmetry; auto.
+assert (exists GH, exists GT, G1 & (w'', Gamma'') = GH & (w, Gamma) ++ GT).
+  apply PPermut_split_neq with (w:=w') (G':=G) (Gamma:=Gamma');
+  try symmetry; auto. transitivity (G1 & (w', Gamma') & (w'', Gamma'')); auto.
+assert (exists GH, exists GT, G1 = GH & (w, Gamma) ++ GT).
+  destruct H6 as (GH, H6); destruct H6 as (GT, H6); subst.
+  apply PPermut_split_neq with (w:=w'') (G':=GH++GT) (Gamma:=Gamma''); auto.
+  rewrite H6; rew_app; auto.
+  right; intro; subst; elim H4; reflexivity.
+destruct H7 as (GH, H7); destruct H7 as (GT, H7); subst.
 apply t_letdia_get_LF with (L_w:=L_w \u \{w''}) 
   (L_t:=L_t) (A:=A) (G:=GH++GT & (w', Gamma'++Gamma'')) (Gamma:=Gamma).
 skip. (* ok_Bg *)
-eapply IHHT with (w1:=w) (G0:=GH++GT & (w0, Gamma0)) (Gamma':=Gamma') (Gamma'':=Gamma''); eauto.
-subst; permut_simpl. skip. (* H0 + H1 *)
-permut_simpl.
+eapply IHHT with (w1:=w) (G0:=GH++GT & (w0, Gamma0)) (Gamma':=Gamma') (Gamma'':=Gamma''); auto.
+rew_app in *. transitivity ((GH ++ GT ++ (w', Gamma') :: (w'', Gamma'') :: nil) & (w0, Gamma0)). apply PPermut_last; auto. apply PPermut_last_rev_simpl with (a:=(w, Gamma)).
+rewrite H5. symmetry. transitivity (GH ++ GT ++ (w, Gamma) :: (w', Gamma') :: (w'', Gamma'') :: nil). rew_app; auto. apply PPermut_app_head; symmetry; auto.
+rew_app; auto.
+rew_app; auto.
 intros. 
-rewrite notin_union in H6; destruct H6.
-rewrite notin_singleton in H7.
 unfold open_var in *; unfold open_ctx in *.
 rewrite <- subst_ctx_comm.
 rewrite subst_order_irrelevant_free.
-eapply H with (G0:=(w'0, (v', A) :: nil) :: (GH ++ GT) & (w, Gamma)); eauto.
-permut_simpl. skip. (* H0 + H1 *)
-permut_simpl.
+eapply H with (G0:=(w'0, (v', A) :: nil) :: (GH ++ GT) & (w, Gamma)) (Gamma':=Gamma') (Gamma'':=Gamma''); auto.
+rew_app in *; constructor; auto.
+transitivity (GH ++ (w, Gamma) :: GT ++ (w', Gamma') :: (w'', Gamma'') :: nil); auto.
+rew_app in *; constructor; auto.
 simpl; auto.
-intro; subst; elim H7; auto.
-subst; permut_simpl.
-apply permut_sym. 
-skip. (*trans with H2 *)
+rewrite notin_union in H8; rewrite notin_singleton in H8; destruct H8.
+intro; subst; elim H9; auto.
+rew_app; symmetry; transitivity ((GH & (w, Gamma) ++ GT) & (w', Gamma'++ Gamma''));
+[ | rew_app]; auto.
 Admitted. (* "No more subgoals but non-instantiated existential variables" *)
 
 Lemma rename_w_preserv_types_new:
 forall G w Gamma A M G' w' Gamma'
   (HT: G |= (w, Gamma) |- M ::: A)
-  (GG': permut G (G' & (w', Gamma'))),
+  (GG': PPermut G (G' & (w', Gamma'))),
   G' |= (w, Gamma ++ Gamma') |- {{ fctx w // fctx w' }} M ::: A.
 intros;
 apply rename_w_preserv_types with (G := G) (w := w) (w':= w'); eauto.
@@ -972,7 +1368,7 @@ Qed.
 Lemma rename_w_preserv_types_old:
 forall G w Gamma A M G' w' Gamma'
   (HT: G |= (w, Gamma) |- M ::: A)
-  (GG': permut G (G' & (w', Gamma'))),
+  (GG': PPermut G (G' & (w', Gamma'))),
   G' |= (w', Gamma' ++ Gamma) |- {{ fctx w' // fctx w }} M ::: A.
 intros;
 apply rename_w_preserv_types with (G := G) (w := w) (w':= w'); eauto.
@@ -981,8 +1377,8 @@ Qed.
 Lemma rename_w_preserv_types_outer:
 forall G G0 w Gamma A M G' w' Gamma' w'' Gamma''
   (HT: G |= (w, Gamma) |- M ::: A)
-  (GG: permut G (G0 & (w', Gamma') & (w'', Gamma'')))
-  (GG': permut G' (G0 & (w', Gamma' ++ Gamma''))),
+  (GG: PPermut G (G0 & (w', Gamma') & (w'', Gamma'')))
+  (GG': PPermut G' (G0 & (w', Gamma' ++ Gamma''))),
   G' |= (w, Gamma) |- {{ fctx w' // fctx w'' }} M ::: A.
 intros;
 eapply rename_w_preserv_types;
@@ -1093,7 +1489,7 @@ forall G M N A w
   (HS: (M, fctx w) |-> (N, fctx w)),
   emptyEquiv G |= (w, nil) |- N ::: A.
 intros;
-remember (w, (@nil (var * ty_LF))) as Ctx;
+remember (w, (@nil (var * ty))) as Ctx;
 remember (emptyEquiv G) as G';
 generalize dependent w;
 generalize dependent N;
@@ -1120,9 +1516,9 @@ unfold open_ctx in *;
 replace ({{fctx w0 // bctx 0}}M0)
   with ({{fctx w0 // fctx w_fresh}} {{fctx w_fresh // bctx 0}}M0)
   by (rewrite subst_ctx_neutral_free; auto);
-replace (@nil (var * ty_LF)) with (nil ++ (@nil (var * ty_LF))); eauto;
+replace (@nil (var * ty)) with (nil ++ (@nil (var * ty))); eauto;
 apply rename_w_preserv_types_old with (G := emptyEquiv G0 & (w0, nil));
-eauto.
+auto.
 (* unbox_fetch_box *)
 inversion HT; subst;
 assert (exists v, v \notin L \u (free_worlds_LF M0)) as HF by apply Fresh;
@@ -1131,15 +1527,14 @@ unfold open_ctx in *;
 replace ({{fctx w0 // bctx 0}}M0)
   with ({{fctx w0 // fctx w_fresh}} {{fctx w_fresh // bctx 0}}M0)
   by (rewrite subst_ctx_neutral_free; auto);
-replace (@nil (var * ty_LF)) with (nil ++ (@nil (var * ty_LF))); eauto;
+replace (@nil (var * ty)) with (nil ++ (@nil (var * ty))); eauto;
 apply rename_w_preserv_types_old with (G := G & (w0, nil) & (w, Gamma));
-try permut_simpl;
-eauto.
+auto.
 (* unbox_fetch *)
 econstructor; eauto;
 (* TODO: permut (G & (w, Gamma)) (emptyEquiv G0) -> Gamma = nil *)
 assert (Gamma = nil) by skip; subst;
-eapply IHHT with (G0:=G & (w0, nil)); eauto;
+eapply IHHT with (G0:=G & (w0, nil)); eauto.
 (* TODO: by H, G contains no Gammas <> nil, so taking emptyEquiv doesn't change anything *)
 skip.
 (* get_here *)
@@ -1164,9 +1559,9 @@ apply subst_t_preserv_types_inner with (A:=A); eauto.
 replace ((v_fresh, A) :: nil) with (nil ++ (v_fresh, A) :: nil) by auto.
 apply rename_w_preserv_types_new with (G:= (w_fresh, (v_fresh, A)::nil) :: emptyEquiv G0).
 rewrite <- subst_order_irrelevant_bound.
-eapply HT2; eauto.
+eapply HT2; auto.
 constructor.
-permut_simpl.
+rew_app; auto.
 skip. (* double emptyEquiv *)
 apply subst_var_preserv_free_worlds; auto.
 constructor.
@@ -1177,20 +1572,21 @@ unfold open_var in *; unfold open_ctx in *.
 rewrite subst_var_neutral_free with (v:=v_fresh).
 rewrite subst_order_irrelevant_bound.
 rewrite <- subst_ctx_neutral_free with (w0:=w_fresh).
-eapply subst_t_preserv_types_outer with (A:=A) (G0:=G) (Gamma':=Gamma) (w':=w); eauto.
-apply permut_sym; assumption.
+eapply subst_t_preserv_types_outer with (A:=A) (G0:=G) (Gamma':=Gamma) (w':=w); auto.
+symmetry; auto.
 skip. (* permut + assumption *)
 apply rename_w_preserv_types_outer with (G0:=G) (Gamma'':=(v_fresh,A) :: nil) 
       (Gamma':=Gamma) (G:=G & (w, Gamma) & (w_fresh, (v_fresh,A)::nil)).
 replace (G & (w, Gamma) & (w_fresh, (v_fresh, A) :: nil)) with ((w_fresh, (v_fresh, A) :: nil) :: emptyEquiv G0) by skip. (* H9 + permut_equiv *)
 rewrite <- subst_order_irrelevant_bound.
-eapply HT2; eauto.
+eapply HT2; auto.
 constructor.
-permut_simpl.
-permut_simpl; skip. (* this is really permutation of permutations *)
+rew_app; auto.
+rew_app. apply PPermut_last; [permut_simpl | ]; auto.
 apply subst_var_preserv_free_worlds; auto.
 constructor.
 apply subst_world_preserv_free_vars; auto.
+
 assert (exists w1, w1 \notin L_w \u free_worlds_LF N) as HF by apply Fresh;
 assert (exists v1, v1 \notin L_t \u free_vars_LF N) as HF2 by apply Fresh;
 destruct HF as (w_fresh); destruct HF2 as (v_fresh);
@@ -1202,7 +1598,7 @@ rewrite subst_var_neutral_free with (v:=v_fresh).
 rewrite subst_order_irrelevant_bound.
 rewrite <- subst_ctx_neutral_free with (w0:=w_fresh).
 eapply subst_t_preserv_types_outer with (A:=A) (G0:=G) (w':=w) (Gamma':=Gamma); eauto.
-apply permut_sym;auto.
+symmetry; auto.
 skip. (* permut + auto *)
 assert (Gamma = nil) by skip; subst. (* H0 *)
 eapply rename_w_preserv_types_outer
@@ -1211,8 +1607,8 @@ eapply rename_w_preserv_types_outer
 rewrite <- subst_order_irrelevant_bound.
 eapply HT2; eauto.
 constructor.
-permut_simpl.
-permut_simpl.
+auto.
+rew_app; auto.
 apply subst_var_preserv_free_worlds; auto.
 constructor.
 apply subst_world_preserv_free_vars; auto.
@@ -1237,21 +1633,22 @@ rewrite subst_order_irrelevant_bound.
 rewrite <- subst_ctx_neutral_free with (w0:=w_fresh).
 replace ((v_fresh,A)::nil) with (nil++(v_fresh,A)::nil) by auto.
 apply rename_w_preserv_types_new with (G:= (w_fresh, (v_fresh,A)::nil) :: G0 & (w, nil));
-eauto.
+auto.
 rewrite <- subst_order_irrelevant_bound.
-eapply HT2; eauto.
+eapply HT2; auto.
 constructor.
-permut_simpl.
 apply subst_var_preserv_free_worlds; auto.
 constructor.
 skip. (* emptyEquiv (emptyEquiv.. ) *)
 apply subst_world_preserv_free_vars; auto.
 (* <> --> exists GH, exists GT, G = GH & (w1, Gamma0) ++ GT *)
-assert (exists GH, exists GT, G = GH & (w1, Gamma0) ++ GT) by skip;
+assert (Gamma0 = nil) by skip; subst Gamma0. (* H0 + H12 *)
+assert (exists GH, exists GT, G = GH & (w1, nil) ++ GT).
+  apply PPermut_split_neq with (w:=w0) (G':=G0) (Gamma:=nil).
+  symmetry; auto.
+  right; intro; subst; elim n; reflexivity.
 destruct H12 as (GH, H12); 
 destruct H12 as (GT, H12).
-assert (Gamma0 = nil) by skip; subst Gamma0. (* H0 + H12 *)
-
 rewrite subst_var_neutral_free with (v:=v_fresh).
 apply subst_t_preserv_types_outer 
   with (A:=A) 
@@ -1259,10 +1656,10 @@ apply subst_t_preserv_types_outer
        (G  := GH ++ GT & (w,nil) & (w1, (v_fresh, A) :: nil)) 
        (G' := GH ++ GT & (w,nil) & (w0, nil))
        (w' :=w1) 
-       (Gamma':=nil);
-try (subst; permut_simpl);
-eauto.
-subst.
+       (Gamma':=nil); auto.
+rew_app; auto.
+rew_app; auto.
+subst; rew_app; auto.
 skip. (* emptyEquiv redundant, H10 + HT0 *)
 
 rewrite subst_order_irrelevant_bound.
@@ -1271,13 +1668,16 @@ apply rename_w_preserv_types_outer
   with (G0 := GH ++ GT & (w,nil)) 
        (G := (w_fresh, (v_fresh, A) :: nil) :: G & (w, nil)) 
        (Gamma':=nil)
-       (Gamma'':=(v_fresh, A)::nil);
-eauto.
+       (Gamma'':=(v_fresh, A)::nil); auto.
 rewrite <- subst_order_irrelevant_bound.
 eapply HT2; eauto.
 constructor.
-subst; permut_simpl.
-permut_simpl.
+subst; rew_app. 
+transitivity ((w_fresh, (v_fresh, A) :: nil) :: GH ++ GT ++ (w, nil) :: (w1, nil) :: nil);
+auto.
+transitivity ((GH ++ GT ++ (w, nil) :: (w1, nil) :: nil) & (w_fresh, (v_fresh, A) :: nil)).
+auto. rew_app; auto.
+rew_app; auto.
 apply subst_var_preserv_free_worlds; auto.
 constructor.
 apply subst_world_preserv_free_vars; auto.
@@ -1287,8 +1687,9 @@ subst; skip. (* contradiction in Ok_Bg*)
 assert (Gamma = nil) by skip. (* from permut *)
 subst.
 replace (emptyEquiv G1) with (G & (w, nil)) by skip. (* permut *)
-econstructor; eauto;
-skip. 
+eapply t_letdia_get_LF ; eauto.
+apply IHHT with (G0:=G & (w0,nil)) (w1:=w); auto.
+skip.
 Qed.
 
 End Lemmas.
